# baseURI: http://www.w3.org/ns/sosa/om
# imports: http://def.isotc211.org/iso19156/2011/SpatialSamplingFeature
# imports: http://def.isotc211.org/iso19156/2011/Specimen
# imports: http://www.w3.org/ns/sosa/
# prefix: sosa-om

@prefix base: <http://def.isotc211.org/iso19150-2/2012/base#> .
@prefix dcterms: <http://purl.org/dc/terms/> .
@prefix iso19156-gfi: <http://def.isotc211.org/iso19156/2011/GeneralFeatureInstance#> .
@prefix iso19156-om: <http://def.isotc211.org/iso19156/2011/Observation#> .
@prefix iso19156-sf: <http://def.isotc211.org/iso19156/2011/SamplingFeature#> .
@prefix iso19156-sfs: <http://def.isotc211.org/iso19156/2011/SpatialSamplingFeature#> .
@prefix iso19156-sp: <http://def.isotc211.org/iso19156/2011/Specimen#> .
@prefix iso19156_gfi: <http://def.isotc211.org/iso19156/2011/GeneralFeatureInstance#> .
@prefix iso19156_sf: <http://def.isotc211.org/iso19156/2011/SamplingFeature#> .
@prefix owl: <http://www.w3.org/2002/07/owl#> .
@prefix rdf: <http://www.w3.org/1999/02/22-rdf-syntax-ns#> .
@prefix rdfs: <http://www.w3.org/2000/01/rdf-schema#> .
@prefix sosa: <http://www.w3.org/ns/sosa/> .
@prefix sosa-om: <http://www.w3.org/ns/sosa/om#> .
@prefix xsd: <http://www.w3.org/2001/XMLSchema#> .
@prefix foaf: <http://xmlns.com/foaf/0.1/>.

dcterms:creator a owl:AnnotationProperty .
dcterms:created a owl:AnnotationProperty .
dcterms:modified a owl:AnnotationProperty .
dcterms:rights a owl:AnnotationProperty .
dcterms:license a owl:AnnotationProperty .
foaf:Agent a owl:Class .
foaf:name a owl:AnnotationProperty .


sosa:om
  rdf:type owl:Ontology ;
  dcterms:creator [ a foaf:Agent ; foaf:name "W3C/OGC Spatial Data on the Web Working Group"@en ] ;
  dcterms:rights "Copyright 2017 W3C/OGC." ;
  dcterms:license <http://www.w3.org/Consortium/Legal/2015/copyright-software-and-document> ;
  dcterms:license <http://www.opengeospatial.org/ogc/Software> ;
  dcterms:creator "Simon J D COX" ;
  dcterms:created "2016-12-14"^^xsd:date ;
  dcterms:creator <http://orcid.org/0000-0002-3884-3420> ;
  dcterms:modified "2017-01-27"^^xsd:date ;
  rdfs:comment """Alignment of the official OWL implementation of ISO 19156 O&M with the W3C/OGC SOSA Ontology;

The official OWL implementation of ISO 19156 O&M was generated automatically from the UML following the rules described in ISO 19150-2 
It is available from the official ISO/TC 211 repository at https://github.com/ISO-TC211/GOM/tree/master/isotc211_GOM_harmonizedOntology 
The ontology itself diverges considerably from idiomatic OWL. 
However, it does provide a canonical URIs for each class and property from the UML model."""@en ;
  rdfs:comment "This graph is provisional. It is the work of only one person and is provided to allow evaluation and support discussion of the potential modularization approach." ;
  rdfs:label "Alignment of ISO 19156 O&M with SOSA"@en ;
  rdfs:seeAlso <http://www.iso.org/iso/catalogue_detail.htm?csnumber=32574> ;
  rdfs:seeAlso <http://www.iso.org/iso/home/store/catalogue_tc/catalogue_detail.htm?csnumber=57466> ;
  rdfs:seeAlso <http://www.opengeospatial.org/standards/om> ;
  rdfs:seeAlso <https://github.com/ISO-TC211/GOM/tree/master/isotc211_GOM_harmonizedOntology> ;
  owl:imports <http://def.isotc211.org/iso19156/2011/SpatialSamplingFeature> ;
  owl:imports <http://def.isotc211.org/iso19156/2011/Specimen> ;
  owl:imports sosa: ;
.

iso19156-om:OM_Observation
  owl:equivalentClass sosa:Observation ;
.
<http://def.isotc211.org/iso19156/2011/Observation#OM_Observation.featureOfInterest>
  owl:equivalentProperty sosa:hasFeatureOfInterest ;
.
<http://def.isotc211.org/iso19156/2011/Observation#OM_Observation.observedProperty>
  owl:equivalentProperty sosa:observedProperty ;
.
<http://def.isotc211.org/iso19156/2011/Observation#OM_Observation.phenomenonTime>
  owl:equivalentProperty sosa:phenomenonTime ;
.
<http://def.isotc211.org/iso19156/2011/Observation#OM_Observation.procedure>
  rdfs:comment "sosa:usedProcedure covers actuation, observation and sampling, so observation procedure is a sub-property" ;
  rdfs:subPropertyOf sosa:usedProcedure ;
.
<http://def.isotc211.org/iso19156/2011/Observation#OM_Observation.result>
  rdfs:comment "sosa:result covers actuation, observation and sampling, so observation result is a sub-property" ;
  rdfs:subPropertyOf sosa:hasResult ;
.
<http://def.isotc211.org/iso19156/2011/Observation#OM_Observation.resultTime>
  rdfs:comment "sosa:resultTime covers actuation, observation and sampling, so observation result time is a sub-property" ;
  rdfs:subPropertyOf sosa:resultTime ;
.
iso19156-om:OM_Process
  rdfs:comment "sosa:Procedure includes procedures for actuation, sampling and observation, so om:Process is the union of a subclass and Sensor" ;
  owl:equivalentClass [
      rdf:type owl:Class ;
      owl:unionOf (
          sosa:Sensor
          sosa-om:ObservationProcedure
        ) ;
    ] ;
.
iso19156_sf:SF_SamplingFeature
  owl:equivalentClass sosa:Sample ;
.
<http://def.isotc211.org/iso19156/2011/SamplingFeature#SF_SamplingFeature.sampledFeature>
  owl:equivalentProperty sosa:isSampleOf ;
.
<http://def.isotc211.org/iso19156/2011/SpatialSamplingFeature#SF_SpatialSamplingFeature.hostedProcedure>
  rdfs:subPropertyOf sosa:hosts ;
.
iso19156-sp:PreparationStep
  rdfs:subClassOf sosa:Sampling ;
.
<http://def.isotc211.org/iso19156/2011/Specimen#PreparationStep.processingDetails>
  rdfs:subPropertyOf sosa:isResultOf ;
.
<http://def.isotc211.org/iso19156/2011/Specimen#PreparationStep.time>
  rdfs:subPropertyOf sosa:resultTime ;
.
iso19156-sp:SF_Process
  rdfs:comment "sosa:Procedure includes procedures for actuation, sampling and observation, so sam:Process is the union of a subclass and SamplingDevice" ;
  owl:equivalentClass [
      rdf:type owl:Class ;
      owl:unionOf (
          sosa:Sampler
          sosa-om:SamplingProcedure
        ) ;
    ] ;
.
<http://def.isotc211.org/iso19156/2011/Specimen#SF_Specimen.samplingMethod>
  rdfs:subPropertyOf sosa:usedProcedure ;
.
<http://def.isotc211.org/iso19156/2011/Specimen#SF_Specimen.samplingTime>
  rdfs:subPropertyOf sosa:resultTime ;
.
sosa:Actuator
  rdfs:subClassOf iso19156_gfi:GFI_Feature ;
.
sosa:FeatureOfInterest
  rdfs:subClassOf iso19156_gfi:GFI_DomainFeature ;
.
sosa:Platform
  rdfs:subClassOf iso19156_gfi:GFI_Feature ;
.
sosa:Procedure
  rdfs:comment "OM_Process and SF_Process each cover both recipes and implementations, so sosa:Procedure is a union of the subsets" ;
  owl:equivalentClass [
      rdf:type owl:Class ;
      owl:disjointUnionOf (
          sosa-om:ActuationProcedure
          sosa-om:ObservationProcedure
          sosa-om:SamplingProcedure
        ) ;
    ] ;
.
sosa-om:ActuationProcedure
  rdf:type owl:Class ;
  rdfs:comment "(Notional) Actuation procedure or recipe, complementing SamplingProcedure and ObservationProcedure"@en ;
  rdfs:label "Actuation procedure"@en ;
  rdfs:subClassOf sosa:Procedure ;
  owl:disjointWith sosa-om:ObservationProcedure ;
  owl:disjointWith sosa-om:SamplingProcedure ;
.
sosa-om:ObservationProcedure
  rdf:type owl:Class ;
  rdfs:comment "(Notional) Observation or sensing procedure or recipe, complementing SamplingProcedure and ActuationProcedure"@en ;
  rdfs:label "Observation procedure"@en ;
  rdfs:subClassOf iso19156-om:OM_Process ;
  rdfs:subClassOf sosa:Procedure ;
  owl:disjointWith sosa-om:ActuationProcedure ;
  owl:disjointWith sosa-om:SamplingProcedure ;
.
sosa-om:SamplingProcedure
  rdf:type owl:Class ;
  rdfs:comment "(Notional) Sampling or sample preparation or processing procedure or recipe, complementing ObservationProcedure and ActuationProcedure"@en ;
  rdfs:label "Sampling procedure"@en ;
  rdfs:subClassOf iso19156-sp:SF_Process ;
  rdfs:subClassOf sosa:Procedure ;
  owl:disjointWith sosa-om:ActuationProcedure ;
  owl:disjointWith sosa-om:ObservationProcedure ;
.
