# baseURI: http://www.w3.org/ns/ssn/ext
# imports: http://www.w3.org/ns/ssn/

@prefix dcterms: <http://purl.org/dc/terms/> .
@prefix ex: <http://example.org/> .
@prefix owl: <http://www.w3.org/2002/07/owl#> .
@prefix rdf: <http://www.w3.org/1999/02/22-rdf-syntax-ns#> .
@prefix rdfs: <http://www.w3.org/2000/01/rdf-schema#> .
@prefix schema: <http://schema.org/> .
@prefix sh: <http://www.w3.org/ns/shacl#> .
@prefix skos: <http://www.w3.org/2004/02/skos/core#> .
@prefix sosa: <http://www.w3.org/ns/sosa/> .
@prefix ssn: <http://www.w3.org/ns/ssn/> .
@prefix ssn-ext: <http://www.w3.org/ns/ssn/ext/> .
@prefix time: <http://www.w3.org/2006/time#> .
@prefix xsd: <http://www.w3.org/2001/XMLSchema#> .

sosa:Actuation
  rdfs:subClassOf [
      a owl:Restriction ;
      owl:minCardinality "1"^^xsd:nonNegativeInteger ;
      owl:onProperty sosa:hasUltimateFeatureOfInterest ;
    ] ;
.
sosa:Observation
  rdfs:comment """If values are not provided for the following Observation properties, they may be provided by the ObservationCollection of which it is a member:
- hasFeatureOfInterest
- hasUltimateFeatureOfInterest
- madeBySensor
- observedProperty
- phenomenonTime
- resultTime
- usedProcedure""" ;
  rdfs:subClassOf [
      a owl:Restriction ;
      owl:minCardinality "1"^^xsd:nonNegativeInteger ;
      owl:onProperty sosa:hasUltimateFeatureOfInterest ;
    ] ;
.
sosa:ObservationCollection
  a owl:Class ;
  rdfs:comment "Collection of observations, typically with one or more property shared by all of its members" ;
  rdfs:label "Collection of observations" ;
  rdfs:subClassOf [
      a owl:Restriction ;
      owl:allValuesFrom sosa:FeatureOfInterest ;
      owl:onProperty sosa:hasFeatureOfInterest ;
    ] ;
  rdfs:subClassOf [
      a owl:Restriction ;
      owl:allValuesFrom sosa:FeatureOfInterest ;
      owl:onProperty sosa:hasUltimateFeatureOfInterest ;
    ] ;
  rdfs:subClassOf [
      a owl:Restriction ;
      owl:allValuesFrom sosa:Property ;
      owl:onProperty sosa:Property ;
    ] ;
  rdfs:subClassOf [
      a owl:Restriction ;
      owl:allValuesFrom sosa:Procedure ;
      owl:onProperty sosa:usedProcedure ;
    ] ;
  rdfs:subClassOf [
      a owl:Restriction ;
      owl:allValuesFrom sosa:Sensor ;
      owl:onProperty sosa:madeBySensor ;
    ] ;
  rdfs:subClassOf [
      a owl:Restriction ;
      owl:allValuesFrom ssn:Stimulus ;
      owl:onProperty ssn:wasOriginatedBy ;
    ] ;
  rdfs:subClassOf [
      a owl:Restriction ;
      owl:maxCardinality "1"^^xsd:nonNegativeInteger ;
      owl:onProperty sosa:hasFeatureOfInterest ;
    ] ;
  rdfs:subClassOf [
      a owl:Restriction ;
      owl:maxCardinality "1"^^xsd:nonNegativeInteger ;
      owl:onProperty sosa:hasUltimateFeatureOfInterest ;
    ] ;
  rdfs:subClassOf [
      a owl:Restriction ;
      owl:maxCardinality "1"^^xsd:nonNegativeInteger ;
      owl:onProperty sosa:madeBySensor ;
    ] ;
  rdfs:subClassOf [
      a owl:Restriction ;
      owl:maxCardinality "1"^^xsd:nonNegativeInteger ;
      owl:onProperty sosa:observedProperty ;
    ] ;
  rdfs:subClassOf [
      a owl:Restriction ;
      owl:maxCardinality "1"^^xsd:nonNegativeInteger ;
      owl:onProperty sosa:phenomenonTime ;
    ] ;
  rdfs:subClassOf [
      a owl:Restriction ;
      owl:maxCardinality "1"^^xsd:nonNegativeInteger ;
      owl:onProperty sosa:resultTime ;
    ] ;
  rdfs:subClassOf [
      a owl:Restriction ;
      owl:maxCardinality "1"^^xsd:nonNegativeInteger ;
      owl:onProperty sosa:usedProcedure ;
    ] ;
  rdfs:subClassOf [
      a owl:Restriction ;
      owl:minCardinality "1"^^xsd:nonNegativeInteger ;
      owl:onProperty sosa:hasMember ;
    ] ;
.
sosa:Sample
  rdfs:subClassOf [
      a owl:Restriction ;
      owl:maxCardinality "1"^^xsd:nonNegativeInteger ;
      owl:onProperty sosa:hasOriginalSample ;
    ] ;
  rdfs:subClassOf [
      a owl:Restriction ;
      owl:minCardinality "1"^^xsd:nonNegativeInteger ;
      owl:onProperty sosa:hasSampledFeature ;
    ] ;
.
sosa:Sampling
  rdfs:subClassOf [
      a owl:Restriction ;
      owl:minCardinality "1"^^xsd:nonNegativeInteger ;
      owl:onProperty sosa:hasUltimateFeatureOfInterest ;
    ] ;
.
sosa:hasFeatureOfInterest
  schema:domainIncludes sosa:ObservationCollection ;
.
sosa:hasMember
  a owl:ObjectProperty ;
  schema:domainIncludes sosa:ObservationCollection ;
  schema:rangeIncludes sosa:Observation ;
  schema:rangeIncludes sosa:ObservationCollection ;
  rdfs:comment "Link to a member within a collection of (observations) or (collections of observations) that share the same value for one or more of the characteristic properties" ;
  rdfs:domain sosa:ObservationCollection ;
  rdfs:label "member observation" ;
  rdfs:range [
      a owl:Class ;
      owl:unionOf (
          sosa:Observation
          sosa:ObservationCollection
        ) ;
    ] ;
  rdfs:subPropertyOf rdfs:member ;
.
sosa:hasOriginalSample
  a owl:ObjectProperty ;
  schema:domainIncludes sosa:Sample ;
  schema:rangeIncludes sosa:Sample ;
  rdfs:comment "link to the original sample that is related to the context sample through a chain of isSampleOf relations" ;
  rdfs:domain sosa:Sample ;
  rdfs:label "has original sample" ;
  rdfs:range sosa:Sample ;
.
sosa:hasSampledFeature
  a owl:ObjectProperty ;
  schema:domainIncludes sosa:Sample ;
  schema:rangeIncludes sosa:FeatureOfInterest ;
  rdfs:comment "link to the ultimate feature of interest of the context sample - i.e. the end of a chain of isSampleOf relations" ;
  rdfs:domain sosa:Sample ;
  rdfs:label "is ultimate sample of" ;
  rdfs:range sosa:FeatureOfInterest ;
.
sosa:hasUltimateFeatureOfInterest
  a owl:ObjectProperty ;
  schema:domainIncludes sosa:Actuation ;
  schema:domainIncludes sosa:Observation ;
  schema:domainIncludes sosa:Sampling ;
  schema:rangeIncludes sosa:FeatureOfInterest ;
  rdfs:comment "link to the ultimate feature of interest of an observation or act of sampling. This is useful when the proximate feature of interest is a sample of the ultimate feature of interest, directly or trasntitively." ;
  rdfs:comment """should match a property chain something like this but with sosa:isSampleOf*
      owl:propertyChainAxiom ( sosa:hasFeatureOfInterest sosa:isSampleOf )""" ;
  rdfs:domain [
      a owl:Class ;
      owl:unionOf (
          sosa:Observation
          sosa:Sampling
          sosa:Actuation
        ) ;
    ] ;
  rdfs:label "has ultimate feature of interest" ;
  rdfs:range sosa:FeatureOfInterest ;
.
sosa:madeBySensor
  schema:domainIncludes sosa:ObservationCollection ;
.
sosa:observedProperty
  schema:domainIncludes sosa:ObservationCollection ;
.
sosa:phenomenonTime
  schema:domainIncludes sosa:ObservationCollection ;
.
sosa:resultTime
  schema:domainIncludes sosa:ObservationCollection ;
.
sosa:usedProcedure
  schema:domainIncludes sosa:ObservationCollection ;
.
ssn:ext
  a owl:Ontology ;
  dcterms:created "2018-03-08"^^xsd:date ;
  dcterms:creator <http://orcid.org/0000-0002-3884-3420> ;
  dcterms:description """Some extensions to the SSN Ontology, to support

1. discovery and use of observation and sample data through links to an ultimate feature-of-interest, or sample
2. observations are  made as part of a set or collection, in which one or more of the observation properties - hasFeatureOfInterest, observedProperty, madeBySensor, usedProcedure, phenomenonTime, resultTime - are shared by all members of the collection. 

These extensions to the SSN Ontology are packaged in a separate RDF graph to enable loading and use if required. """ ;
  dcterms:license <http://www.opengeospatial.org/ogc/Software> ;
  dcterms:license <http://www.w3.org/Consortium/Legal/2015/copyright-software-and-document> ;
  dcterms:modified "2019-12-24"^^xsd:date ;
  dcterms:rights "Copyright 2019 W3C/OGC." ;
  dcterms:title "Extensions to the SSN Ontology"@en ;
  rdfs:comment """The classes, properties, and axioms in this RDF graph are described in https://www.w3.org/TR/vocab-ssn-ext/

Their status is non-normative, and SSN applications are not required to recognize or support them. """ ;
  rdfs:label "SSN extensions" ;
  owl:imports ssn: ;
.
