@prefix rdf:  <http://www.w3.org/1999/02/22-rdf-syntax-ns#> .
@prefix rdfs: <http://www.w3.org/2000/01/rdf-schema#>.
@prefix xsd:  <http://www.w3.org/2001/XMLSchema#> .
@prefix skos: <http://www.w3.org/2004/02/skos/core#> .
@prefix qudt: <http://qudt.org/schema/qudt/> .
@prefix unit: <http://qudt.org/vocab/unit/> .
@prefix foaf: <http://xmlns.com/foaf/0.1/> .
@prefix schema: <http://schema.org/> .
@prefix gs1: <https://gs1.org/voc/> .
@prefix equipment: <https://rdf.ag/o/equipment/> .
@prefix owl: <http://www.w3.org/2002/07/owl#> .
@prefix sosa: <http://www.w3.org/ns/sosa/> .
@prefix ssn: <http://www.w3.org/ns/ssn/> .
@prefix ssn-system: <http://www.w3.org/ns/ssn/systems/> .
@base <https://rdf.ag/o/equipment/> .

# This example is a specification for a common over-the-shelf temperature and humidity sensor. It is a specification
# representing the commercial sensor product from which different instantions can be derived for each specific physical instance of
# the product.
#
# This prevents duplication of the information required for each new physical instance while allowing results to be related to the
# actualy physical device that generated them.
# 

<InkBird-IBS-TH2> a owl:Class, gs1:Product ;
    rdfs:label "Inkbird IBS-TH2"@en ;
    rdfs:subClassOf sosa:Platform, equipment:Equipment, <https://w3id.org/seas/BluetoothCommunicationDevice> ;
    gs1:pip <https://inkbird.com/products/hygrometer-ibs-th2> ;
    sosa:hosts <IBSTH2BatteryVoltageSensor>, <IBSTH2HumiditySensor>, <IBSTH2TemperatureSensor> ;
    sosa:implements <InkBird-IBS-TH2-Procedure> ;
    gs1:brand <InkBird> .

<InkBird> a gs1:Brand ;
    rdfs:label "Inkbird"@en ;
    rdfs:comment "This is a commercial product."@en ;
    gs1:brandName "Inkbird"@en .

<HWAddress> a owl:DatatypeProperty ;
    rdfs:label "Device Hardware Address"@en ;
    rdfs:range <InkBird-IBS-TH2> .

<IBSTH2Battery>
    a owl:Class ;
    rdfs:label "IBSTH2 Battery. 2 AAA Batteries. 3.0V Nominal."@en ;
    skos:definition "A generic description of the battery pack that needs to be installed in it."@en ;
    rdfs:subClassOf sosa:FeatureOfInterest .

<IBSTH2BatteryLimits>
    skos:editorialNote "Of course, we'd never receive a 0% battery reading..."@en ;
    schema:maxValue "100" ;
    schema:minValue "0" ;
    schema:unitCode unit:PERCENT ;
    a schema:PropertyValue, sosa:Property, ssn-system:Accuracy ;
    rdfs:label "IBSTH2 Battery Limits"@en .

<IBSTH2BatteryVoltageSensor> a owl:Class ;
    skos:editorialNote "Percentage is derived from the battery voltage."@en ;
    rdfs:label "IBSTH2 Battery Voltage"@en ;
    rdfs:subClassOf sosa:Sensor ;
    ssn-system:hasOperatingRange <IBSTH2BatteryLimits> ;
    sosa:implements <InkBird-IBS-TH2-Procedure> ;
    sosa:observes <IBSTH2Battery> .

<IBSTH2BatteryHealth>
    schema:unitCode unit:PERCENT ;
    a sosa:ObservableProperty, sosa:Property ;
    rdfs:label "Battery Health"@en ;
    skos:definition "Battery Health expressed as a percentage."@en .


<IBSTH2HumiditySensor> a owl:Class ;
    rdfs:label "Inkbird IBS-TH2 built-in Humidity Sensor"@en ;
    rdfs:subClassOf sosa:Sensor ;
    sosa:observes <airRelativeHumidity> ;
    ssn-system:hasOperatingRange <IBSTH2HumiditySensorLimits>, <IBSTH2TemperatureSensorLimits> ;
    sosa:implements <InkBird-IBS-TH2-Procedure> ;
    ssn-system:hasSystemCapability <IBSTH2HumiditySensorCapability> .

<IBSTH2HumiditySensorAccuracy>
    schema:maxValue "0.5" ;
    schema:minValue "-0.5" ;
    schema:unitCode unit:Percent ;
    a schema:PropertyValue, sosa:Property, ssn-system:Accuracy ;
    skos:definition "The accuracy of the humidity sensor is +-0.5 °C in normal temperature and humidity conditions."@en .

<IBSTH2HumiditySensorCapability>
    a schema:PropertyValue, sosa:Property, ssn-system:SystemCapability ;
    skos:definition "The capabilities of the humidity sensor in normal temperature and humidity conditions."@en ;
    ssn-system:hasSystemProperty <IBSTH2HumiditySensorAccuracy> ;
    ssn-system:inCondition <IBSTH2HumiditySensorNormalLimits>, <IBSTH2TemperatureSensorNormalLimits> .

<IBSTH2HumiditySensorLimits>
    a ssn-system:OperatingRange ;
    rdfs:label "Inkbird IBS-TH2 Humidity Sensor Limits"@en ;
    ssn-system:inCondition <IBSTH2HumiditySensorNormalLimits> .

<IBSTH2HumiditySensorNormalLimits>
    schema:maxValue "100" ;
    schema:minValue "0" ;
    schema:unitCode unit:PERCENT ;
    a schema:PropertyValue, ssn-system:Condition .

<IBSTH2TemperatureSensor>
    a owl:Class ;
    rdfs:label "Inkbird IBS-TH2 built-in Temperature Sensor"@en ;
    rdfs:subClassOf sosa:Sensor ;
    sosa:observes <airTemperature> ;
    ssn-system:hasOperatingRange <IBSTH2HumiditySensorLimits>, <IBSTH2TemperatureSensorLimits> ;
    sosa:implements <InkBird-IBS-TH2-Procedure> ;
    ssn-system:hasSystemCapability <IBSTH2TemperatureSensorCapability> .

<IBSTH2TemperatureSensorAccuracy>
    schema:maxValue "0.5" ;
    schema:minValue "-0.5" ;
    schema:unitCode unit:DEG_C ;
    a schema:PropertyValue, sosa:Property, ssn-system:Accuracy ;
    skos:definition "The accuracy of the temperature sensor is +-0.5 °C in normal temperature and humidity conditions."@en .

<IBSTH2TemperatureSensorCapability>
    a schema:PropertyValue, sosa:Property, ssn-system:SystemCapability ;
    skos:definition "The capabilities of the temperature sensor in normal temperature and humidity conditions."@en ;
    ssn-system:hasSystemProperty <IBSTH2TemperatureSensorAccuracy> ;
    ssn-system:inCondition <IBSTH2HumiditySensorNormalLimits>, <IBSTH2TemperatureSensorNormalLimits> .

<IBSTH2TemperatureSensorLimits>
    a ssn-system:OperatingRange ;
    rdfs:label "Inkbird IBS-TH2 Temperature Sensor Limits"@en ;
    ssn-system:inCondition <IBSTH2TemperatureSensorNormalLimits> .

<IBSTH2TemperatureSensorNormalLimits>
    schema:maxValue "60" ;
    schema:minValue "-40" ;
    schema:unitCode unit:DEG_C ;
    a schema:PropertyValue, ssn-system:Condition .

<InkBird-IBS-TH2-Procedure> a sosa:Procedure ;
  foaf:isPrimaryTopicOf <https://fcc.report/FCC-ID/2AYZD-IBSTH2/5436475.pdf> ;
  skos:editorialNote "This is the manufacturer's data sheet as submitted to the FCC."@en .

<airRelativeHumidity>
    schema:unitCode unit:PERCENT ;
    a sosa:ObservableProperty, sosa:Property ;
    rdfs:label "Humidité Relative"@fr, "Relative Humidity"@en, "Relative Luftfeuchtigkeit"@de ;
    skos:definition "The amount of water vapor present in air expressed as a percentage of the amount needed for saturation at the same temperature."@en .

<airTemperature>
    schema:unitCode unit:DEG_C ;
    a sosa:ObservableProperty, sosa:Property ;
    rdfs:label "Lufttemperatur"@de, "Air Temperature"@en, "Température Ambiante"@fr ;
    skos:definition "Temperature of the air."@en .

