# baseURI: http://example.org/vistavital-a
# imports: http://www.w3.org/2006/time
# imports: http://www.w3.org/ns/prov-o#
# imports: http://www.w3.org/ns/ssn/
# imports: https://raw.githubusercontent.com/schemaorg/schemaorg/master/data/releases/3.3/all-layers.ttl
# prefix: vistavital-a

@prefix dcterms: <http://purl.org/dc/terms/> .
@prefix ex: <http://example.org/> .
@prefix owl: <http://www.w3.org/2002/07/owl#> .
@prefix prov: <http://www.w3.org/ns/prov#> .
@prefix rdf: <http://www.w3.org/1999/02/22-rdf-syntax-ns#> .
@prefix rdfs: <http://www.w3.org/2000/01/rdf-schema#> .
@prefix schema: <http://schema.org/> .
@prefix sosa: <http://www.w3.org/ns/sosa/> .
@prefix time: <http://www.w3.org/2006/time#> .
@prefix vistavital-a: <http://example.org/vistavital-a#> .
@prefix xsd: <http://www.w3.org/2001/XMLSchema#> .

ex:entered-by
  rdf:type owl:ObjectProperty ;
  rdfs:comment "This simple property is defined to be equivalent to prov:qualifiedAssociation with the value of prov:hadRole fixed to \"Entered by\"" ;
  rdfs:label "Data entered by" ;
  rdfs:subPropertyOf prov:wasAssociatedWith ;
  owl:propertyChainAxiom (
      [
        rdf:type owl:ObjectProperty ;
        rdfs:range [
            rdf:type owl:Class ;
            rdfs:subClassOf prov:Association ;
            rdfs:subClassOf [
                rdf:type owl:Restriction ;
                owl:hasValue [
                    rdf:type prov:Role ;
                    rdfs:label "Entered by" ;
                  ] ;
                owl:onProperty prov:hadRole ;
              ] ;
          ] ;
        rdfs:subPropertyOf prov:qualifiedAssociation ;
      ]
      prov:agent
    ) ;
.
ex:error-entered-by
  rdf:type owl:ObjectProperty ;
  rdfs:comment "This simple property is defined to be equivalent to prov:qualifiedAssociation with the value of prov:hadRole fixed to \"Error entered by\"" ;
  rdfs:label "Error entered by" ;
  rdfs:subPropertyOf prov:wasAssociatedWith ;
  owl:propertyChainAxiom (
      [
        rdf:type owl:ObjectProperty ;
        rdfs:range [
            rdf:type owl:Class ;
            rdfs:subClassOf prov:Association ;
            rdfs:subClassOf [
                rdf:type owl:Restriction ;
                owl:hasValue [
                    rdf:type prov:Role ;
                    rdfs:label "Error entered by" ;
                  ] ;
                owl:onProperty prov:hadRole ;
              ] ;
          ] ;
        rdfs:subPropertyOf prov:qualifiedAssociation ;
      ]
      prov:agent
    ) ;
.
ex:vistavital-a
  rdf:type owl:Ontology ;
  dcterms:created "2017-10-18" ;
  dcterms:creator "Simon Cox" ;
  rdfs:comment """This document shows how a vital-signs observation can be represented using SOSA. 
Three variants are included:
1. SOSA + schema.org
2. SOSA + prov-o
3. SOSA + prov-o + customized properties derived from prov-o but which make the serialization more compact 

The example data comes from the Vista example developed by Rafael Richards - see <https://github.com/vistadataproject/documents/blob/master/Background/presentations/pdf/2014-Linked_Vitals-Linked_Data_Linked_FHIR.pdf> """ ;
  rdfs:seeAlso <https://github.com/vistadataproject/documents/blob/master/Background/presentations/pdf/2014-Linked_Vitals-Linked_Data_Linked_FHIR.pdf> ;
  owl:imports <http://www.w3.org/2006/time> ;
  owl:imports <http://www.w3.org/ns/prov-o#> ;
  owl:imports <http://www.w3.org/ns/ssn/> ;
  owl:imports <https://raw.githubusercontent.com/schemaorg/schemaorg/master/data/releases/3.3/all-layers.ttl> ;
.
vistavital-a:Observation_1_ex
  rdf:type sosa:Observation ;
  ex:entered-by <http://example.org/NEW-PERSON/NOTHER,NADA> ;
  ex:error-entered-by <http://example.org/NEW-PERSON/MANAGER,SYSTEM> ;
  schema:status "error" ;
  rdfs:comment "Example of how to encode a Vital Signs measurement comparable to Vista example" ;
  rdfs:comment "This version uses schema.org and prov for elements not available in SOSA, with some locally defined specializations of prov Associations to formally bind roles to simple properties" ;
  rdfs:label "Example BP measurement" ;
  rdfs:seeAlso <https://github.com/vistadataproject/documents/blob/master/Background/presentations/pdf/2014-Linked_Vitals-Linked_Data_Linked_FHIR.pdf> ;
  prov:atLocation <http://example.org/HOSPITAL-LOCATION/4-SOUTH-MED> ;
  sosa:hasFeatureOfInterest <http://example.org/patient/jones-christopher> ;
  sosa:hasResult "150/10" ;
  sosa:observedProperty <VA:4500634> ;
  sosa:observedProperty <http://example.org/GMRV-VITAL-TYPE/BLOOD-PRESSURE> ;
  sosa:phenomenonTime [
      rdf:type time:Instant ;
      time:inXSDDateTime "2005-09-01T13:00:00Z"^^xsd:dateTime ;
    ] ;
  sosa:resultTime "2005-12-28T13:48:44Z"^^xsd:dateTime ;
.
vistavital-a:Observation_1_prov
  rdf:type sosa:Observation ;
  schema:status "error" ;
  rdfs:comment "Example of how to encode a Vital Signs measurement comparable to Vista example" ;
  rdfs:comment "This version uses prov for elements not included in SOSA" ;
  rdfs:label "Example BP measurement" ;
  rdfs:seeAlso <https://github.com/vistadataproject/documents/blob/master/Background/presentations/pdf/2014-Linked_Vitals-Linked_Data_Linked_FHIR.pdf> ;
  prov:atLocation <http://example.org/HOSPITAL-LOCATION/4-SOUTH-MED> ;
  prov:qualifiedAssociation [
      rdf:type prov:Association ;
      prov:agent <http://example.org/NEW-PERSON/MANAGER,SYSTEM> ;
      prov:hadRole [
          rdf:type prov:Role ;
          rdfs:label "Error entered by" ;
        ] ;
    ] ;
  prov:qualifiedAssociation [
      rdf:type prov:Association ;
      prov:agent <http://example.org/NEW-PERSON/NOTHER,NADA> ;
      prov:hadRole [
          rdf:type prov:Role ;
          rdfs:label "Entered by" ;
        ] ;
    ] ;
  sosa:hasFeatureOfInterest <http://example.org/patient/jones-christopher> ;
  sosa:hasResult "150/10" ;
  sosa:observedProperty <VA:4500634> ;
  sosa:observedProperty <http://example.org/GMRV-VITAL-TYPE/BLOOD-PRESSURE> ;
  sosa:phenomenonTime [
      rdf:type time:Instant ;
      time:inXSDDateTime "2005-09-01T13:00:00Z"^^xsd:dateTime ;
    ] ;
  sosa:resultTime "2005-12-28T13:48:44Z"^^xsd:dateTime ;
.
vistavital-a:Observation_1_sdo
  rdf:type sosa:Observation ;
  schema:agent <http://example.org/NEW-PERSON/NOTHER,NADA> ;
  schema:location <http://example.org/HOSPITAL-LOCATION/4-SOUTH-MED> ;
  schema:participant <http://example.org/NEW-PERSON/MANAGER,SYSTEM> ;
  schema:status "error" ;
  rdfs:comment "Example of how to encode a Vital Signs measurement comparable to Vista example" ;
  rdfs:comment "This version uses schema.org elements for elements not part of SOSA" ;
  rdfs:label "Example BP measurement" ;
  rdfs:seeAlso <https://github.com/vistadataproject/documents/blob/master/Background/presentations/pdf/2014-Linked_Vitals-Linked_Data_Linked_FHIR.pdf> ;
  sosa:hasFeatureOfInterest <http://example.org/patient/jones-christopher> ;
  sosa:hasResult "150/10" ;
  sosa:observedProperty <VA:4500634> ;
  sosa:observedProperty <http://example.org/GMRV-VITAL-TYPE/BLOOD-PRESSURE> ;
  sosa:phenomenonTime [
      rdf:type time:Instant ;
      time:inXSDDateTime "2005-09-01T13:00:00Z"^^xsd:dateTime ;
    ] ;
  sosa:resultTime "2005-12-28T13:48:44Z"^^xsd:dateTime ;
.
