@prefix rdf: <http://www.w3.org/1999/02/22-rdf-syntax-ns#> .
@prefix rdfs: <http://www.w3.org/2000/01/rdf-schema#> .
@prefix owl: <http://www.w3.org/2002/07/owl#> .
@prefix xsd: <http://www.w3.org/2001/XMLSchema#> .
@prefix skos: <http://www.w3.org/2004/02/skos/core#> .
@prefix dcterms: <http://purl.org/dc/terms/> .
@prefix foaf: <http://xmlns.com/foaf/0.1/>.
@prefix time: <http://www.w3.org/2006/time#> .

@prefix schema: <http://schema.org/> .

@prefix sosa: <http://www.w3.org/ns/sosa/> .
@prefix sosa-common: <http://www.w3.org/ns/sosa/common/> .


sosa-common: 
  a owl:Ontology ;
  dcterms:title "Sensor, Observation, Sample, and Actuator (SOSA) Ontology - core module"@en ;
  dcterms:description "Core classes and properties for the SSN Ontology."@en ;
  dcterms:creator [ a foaf:Agent ; foaf:name "W3C/OGC Spatial Data on the Web Working Group"@en ] ;
  dcterms:rights "Copyright 2024 W3C/OGC." ;
  dcterms:license <http://www.w3.org/Consortium/Legal/2015/copyright-software-and-document> ;
  dcterms:license <http://www.opengeospatial.org/ogc/Software> ;
  dcterms:created "2024-02-02"^^xsd:date ;
  .


## Utility terms 

sosa:hasMember 
  a owl:ObjectProperty ;
  rdfs:label "has member of collection" ;
  skos:definition """
  Link to a member (actuation or sample or observation) or (collection of actuation or collection of samples or collection of observations) within a collection. 
  """ ;
  skos:scopeNote "rules for the consistency of values of properties of collections and properties of their members are given for each collection type" ;
  skos:editorialNote "Note that there is a single `member` property. OWL or SHACL constraints may limit the range depending on the context of different collection types" ;
  rdfs:isDefinedBy sosa-common: .


## Features of interest and Property

sosa:FeatureOfInterest 
  a owl:Class ;
  rdfs:label "Feature Of Interest"@en ;
  skos:definition """
  The thing that is the target of the Execution, i.e. whose property is being estimated or calculated in the course of an Observation to arrive at a result, or whose property is being manipulated by an Actuator, or which is being sampled or transformed in an act of Sampling.
  """@en ;
  skos:example "When measuring the height of a tree, the height is the observed ObservableProperty, 20m may be the Result of the Observation, and the tree is the FeatureOfInterest. A window is a FeatureOfInterest for an automatic window control Actuator."@en ;
  rdfs:isDefinedBy sosa-common: .

sosa:hasProperty 
  a owl:ObjectProperty ; 
  rdfs:label "has property"@en ;
  skos:definition """
  Relation between an entity and a Property of that entity.
  """@en ;
  schema:domainIncludes sosa:FeatureOfInterest ;
  schema:rangeIncludes sosa:Property ;
  schema:rangeIncludes sosa:PropertyOfInterest ;
  owl:inverseOf sosa:isPropertyOf ;
  rdfs:isDefinedBy sosa-common: .

sosa:isFeatureOfInterestOf 
  a owl:ObjectProperty ;
  rdfs:label "is feature of interest of"@en ;
  skos:definition """
  A relation between a FeatureOfInterest and an Execution concerning it, i.e.an Observation about it, an Actuation acting on it, or an act of Sampling that sampled it.
  """@en ;
  schema:domainIncludes sosa:FeatureOfInterest ;
  schema:rangeIncludes sosa:Execution ;
  owl:inverseOf sosa:hasFeatureOfInterest ;
  rdfs:isDefinedBy sosa-common: .

sosa:Property 
  a owl:Class ;
  rdfs:label "Property"@en ;
  skos:definition """
  An identifiable quality of a FeatureOfInterest that can be observed or acted upon. A property can apply to different features of interest.
  """@en ;
  skos:example "Cars (a feature type) all have a characteristic colour, where 'colour' is a property."@en ;
  skos:note "Concepts from existing code lists, vocabularies, and taxonomies, may be used as instances of Property"@en ;
  rdfs:isDefinedBy sosa-common: .

sosa:PropertyOfInterest 
  a owl:Class ;
  rdfs:label "Property Of Interest"@en ;
  skos:definition """
  An identifiable quality of a specific FeatureOfInterest that can be observed or acted upon. A property of interest is tied to a specific feature of interest. It is inherent to and cannot exist without that FeatureOfInterest.
  """@en ;
  skos:example "Abby's car has the colour red, where \"colour red\" is a property of interest of the car."@en ;
  skos:note "Properties of interest need not always be explicitly identified. It depends on the use case."@en ;
  rdfs:isDefinedBy sosa-common: .

sosa:isPropertyOf 
  a owl:ObjectProperty ;
  rdfs:label "is property of"@en ;
  skos:definition """
  Relation between a Property and the entity that it belongs to.
  """@en ;
  schema:domainIncludes sosa:Property ;
  schema:domainIncludes sosa:PropertyOfInterest ;
  schema:rangeIncludes sosa:FeatureOfInterest ;
  owl:inverseOf sosa:hasProperty ; 
  rdfs:isDefinedBy sosa-common: .

sosa:forProperty 
  a owl:ObjectProperty ;
  rdfs:label "for property"@en ;
  skos:definition """
  A relation between some entity and a Property.
  """@en ;
  skos:example "For example, from a Sensor to the properties it can observe; from an Actuator to the properties it can act on; from a Deployment to the properties it was installed to observe or act on; from a SystemCapability to the Property the capability is described for."@en ;
  schema:domainIncludes sosa:Deployment ;
  schema:domainIncludes sosa:Procedure ;
  schema:domainIncludes sosa:System ;
  schema:rangeIncludes sosa:Property ;
  rdfs:isDefinedBy sosa-common: .


## Procedures

sosa:Procedure 
  a owl:Class ;
  rdfs:label "Procedure"@en ;
  skos:definition """
  A workflow, protocol, plan, algorithm, or computational method specifying how to make a change to the state of the world (through an Actuation) or an Observation, or create a Sample. A Procedure is re-usable, and might be involved in many Actuations, or Observations, or Samplings. It explains the steps to be carried out to arrive at reproducible results.
  """@en ;
  skos:example "The measured wind speed differs depending on the height of the sensor above the surface, e.g., due to friction. Consequently, procedures for measuring wind speed define a standard height for anemometers above ground, typically 10m for meteorological measures and 2m in Agrometeorology. This definition of height, sensor placement, and so forth are defined by the Procedure."@en ;
  skos:note "Many observations may be created via the same Procedure, the same way as many tables are assembled using the same instructions (as information objects, not their concrete realization)."@en ;
  rdfs:isDefinedBy sosa-common: .

sosa:implementedBy 
  a owl:ObjectProperty ;
  rdfs:label "implemented by"@en ;
  skos:definition """
  Relation between a Procedure (an algorithm, procedure or method) and an entity that implements that Procedure in some executable way.
  """@en ;
  skos:example "For example, the relationship between a scientific measuring Procedure and a sensor that senses via that Procedure."@en ;
  schema:domainIncludes sosa:Procedure ;
  schema:rangeIncludes sosa:System ;
  owl:inverseOf sosa:implements ;
  rdfs:isDefinedBy sosa-common: .

sosa:hasInput 
  a owl:ObjectProperty ;
  rdfs:label "has input"@en ;
  skos:definition """
  Relation between a Procedure and an Input to it.
  """@en ;
  schema:domainIncludes sosa:Procedure ;
  rdfs:isDefinedBy sosa-common: .

sosa:hasOutput 
  a owl:ObjectProperty ;
  rdfs:label "has output"@en ;
  skos:definition """
  Relation between a Procedure and an Output of it.
  """@en ;
  schema:domainIncludes sosa:Procedure ;
  rdfs:isDefinedBy sosa-common: .

sosa:hasProcedure 
  a owl:ObjectProperty ;
  rdfs:label "has procedure"@en ;
  skos:definition """
  Relation between a Property and a Procedure that can observe or act on it.
  """@en ;
  schema:domainIncludes sosa:Property ;
  schema:rangeIncludes sosa:Procedure ;
  rdfs:isDefinedBy sosa-common: .

## Executions

sosa:Execution 
  a owl:Class ;
  rdfs:label "Execution of a Procedure"@en ;
  skos:definition """
  Act of carrying out a Procedure. This class generalizes the Observation, Actuation, and Sampling classes. It is not expected to be used directly.
  """@en ;
  rdfs:isDefinedBy sosa-common: .

sosa:usedProcedure 
  a owl:ObjectProperty ;
  rdfs:label "used procedure"@en ;
  skos:definition """
  A relation to link to a re-usable Procedure used in making an Execution (an Observation, an Actuation, or a Sampling), typically using an Actuator, a Sensor, or a Sampler.
  """@en ;
  schema:domainIncludes sosa:Execution ;
  schema:rangeIncludes sosa:Procedure ;
  rdfs:isDefinedBy sosa-common: .

sosa:madeBySystem 
  a owl:ObjectProperty ;
  rdfs:label "made by system"@en ;
  skos:definition """
  Relation linking an Execution to the System that made it.
  """@en ;
  schema:domainIncludes sosa:Execution ;
  schema:rangeIncludes sosa:System ;
  owl:inverseOf sosa:madeExecution ;
  rdfs:isDefinedBy sosa-common: .

sosa:startTime 
  a owl:DatatypeProperty ;
  rdfs:label "start time"@en ;
  skos:definition """
  The instant of time when the Execution was initiated or tasked, i.e. the Actuation or Observation or Sampling 
  """@en ;
  rdfs:comment "The value would usually be encoded using xsd:dateTime xsd:date xsd:gYearMonth xsd:gYear"@en ;
  schema:domainIncludes sosa:Execution ;
  rdfs:isDefinedBy sosa-common: .

sosa:resultTime 
  a owl:DatatypeProperty ;
  rdfs:label "result time"@en ;
  skos:definition """
  The instant of time when the Execution was completed, i.e. the Actuation or Observation or Sampling  
  """@en ;
  rdfs:comment "The value would usually be encoded using xsd:dateTime xsd:date xsd:gYearMonth xsd:gYear"@en ;
  schema:domainIncludes sosa:Execution ;
  rdfs:isDefinedBy sosa-common: .

sosa:phenomenonTime 
  a owl:ObjectProperty ;
  rdfs:label "phenomenon time"@en ;
  skos:definition """
  The time that the result of an Execution (i.e. Actuation, Observation, or Sampling) applies to the FeatureOfInterest. It may be an Interval or an Instant, or some other compound TemporalEntity. 
  """@en ;
  skos:scopeNote """
  The phenomenonTime is not necessarily the same as the resultTime. 
  
  In the case of Actuation, phenomenonTime should indicate the time that the actuator was active. 

  In the case of Observation, the phenomenonTime may be distant from the resultTime, for example in the case of forecasts the phenomenonTime is after the resultTime, and in historical, geological and cosmological investigations the phenomenonTime may be far in the past while the resultTime is contemporary. 

  In the case of Sampling the phenomenonTime should indicate the period during which the Sampling Procedure was active, while the resultTime may indicate when the sample comes into the posession of the operator. 
  """@en ;
  schema:domainIncludes sosa:Execution ;
  schema:rangeIncludes time:TemporalEntity ;
  rdfs:isDefinedBy sosa-common: .

sosa:hasFeatureOfInterest 
  a owl:ObjectProperty ;
  rdfs:label "has feature of interest"@en ;
  skos:definition """
  A relation between an Execution and its target entity, i.e. an Actuation and the entity whose property was modified, or an Observation and the entity whose quality was observed, or an act of Sampling and the entity that was sampled.
  """@en ;
  skos:scopeNote "This is the _proximate_ feature of interest, which may be a proxy entity such as a sample of the _ultimate_ feature of interest. Use `hasUltimateFeatureOfInterest` if the intention is to link to the _ultimate_ feature of interest. " ;
  skos:example "For example, in an Observation of the weight of a person, the FeatureOfInterest is the person and the property is its weight."@en ;
  schema:domainIncludes sosa:Execution ;
  schema:rangeIncludes sosa:FeatureOfInterest ;
  owl:inverseOf sosa:isFeatureOfInterestOf ;
  rdfs:isDefinedBy sosa-common: .

sosa:hasUltimateFeatureOfInterest 
  a owl:ObjectProperty ;
  rdfs:label "has ultimate feature of interest"@en  ;
  skos:definition """
  A relation between an Execution and its ultimate target entity i.e. an Actuation and the ultimate entity whose property was modified, an Observation and the ultimate entity whose quality was observed, or  between an act of Sampling and the ultimate entity that was sampled. 
  """@en ;
  skos:scopeNote "This is useful when the proximate feature of interest is a sample of the ultimate feature of interest, directly or transitively." ;
  skos:note """should match a property chain something like this but with sosa:isSampleOf*
      owl:propertyChainAxiom ( sosa:hasFeatureOfInterest sosa:isSampleOf )""" ;
  schema:domainIncludes sosa:Execution ;
  schema:rangeIncludes sosa:FeatureOfInterest ;
  rdfs:isDefinedBy sosa-common: .

sosa:hasInputValue 
  a owl:ObjectProperty ;
  rdfs:label "has input value"@en ;
  skos:definition """
  Assigns a value to an input defined by the Procedure that is used in an Execution (Actuation, Observation, Sampling).
  """@en ;
  skos:note "The input value should be suitable for the input definition on the corresponding usedProcedure"@en ;
  schema:domainIncludes sosa:Execution ;
  rdfs:isDefinedBy sosa-common: .

sosa:hasOutputValue 
  a owl:ObjectProperty ;
  rdfs:label "has output value"@en ;
  skos:definition """
  Assigns a value to an output defined by the Procedure that is used in an Execution (Actuation, Observation, Sampling).
  """@en ;
  skos:note "The output value should be suitable for the output definition on the corresponding usedProcedure"@en ;
  schema:domainIncludes sosa:Execution ;
  rdfs:isDefinedBy sosa-common: .


## Result 

sosa:Result 
  a owl:Class ;
  owl:deprecated true ;
  rdfs:label "Result"@en ;
  skos:definition """
  The Result of an Observation, Actuation, or act of Sampling. 
  
  To store an observation's simple result value one can use the hasSimpleResult property.
  """@en ;
  skos:example "The value 20 as the height of a certain tree together with the unit, e.g., Meter."@en ;
  rdfs:isDefinedBy sosa-common: .

sosa:hasResult 
  a owl:ObjectProperty ;
  rdfs:label "has result"@en ;
  skos:definition """""
  Relation linking an Execution (i.e. Actuation or Observation or act of Sampling) to its result or Sample.

  In the case of an Actuation, the result is the expected value of the ActuatableProperty following the execution of the Procedure by the Actuator. 

  In the case of an Observation, the result is the value of the ObservableProperty produced by the execution of the Procedure by the Sensor. 
  
  In the case of a Sampling, the result is the Sample produced by the execution of the Procedure by the Sampler. 
  """@en ;
  schema:domainIncludes sosa:Execution ;
  owl:inverseOf sosa:isResultOf ;
  rdfs:isDefinedBy sosa-common: .

sosa:isResultOf 
  a owl:ObjectProperty ;
  rdfs:label "is result of"@en ;
  skos:definition """
  Relation linking a Result to the Execution (i.e. the Actuation or Observation or act of Sampling) that created or caused it.
  """@en ;
  schema:rangeIncludes sosa:Execution ;
  owl:inverseOf sosa:hasResult ;
  rdfs:isDefinedBy sosa-common: .

sosa:hasSimpleResult 
  a owl:DatatypeProperty ;
  rdfs:label "has simple result"@en ;
  skos:definition """
  The simple value of an Actuation or Observation.

  In the case of an Actuation, the result is the expected value of the ActuatableProperty following the execution of the Procedure by the Actuator. 

  In the case of an Observation, the result is the value of the ObservableProperty produced by the execution of the Procedure by the Sensor. 
  """@en ;
  skos:example "For instance, the values 23 or true."@en ;
  schema:domainIncludes sosa:Execution ;
  rdfs:isDefinedBy sosa-common: .


## Systems

sosa:System 
  a owl:Class ;
  rdfs:label "System"@en ;
  skos:definition """
  System is a unit of abstraction for pieces of infrastructure that implement Procedures. A System may have components, its subsystems, which are other systems.
  """@en ; 
  rdfs:isDefinedBy sosa-common: .

sosa:implements 
  a owl:ObjectProperty ;
  rdfs:label "implements"@en ;
  skos:definition """
  Relation between an entity that implements a Procedure in some executable way and the Procedure (an algorithm, procedure or method).
  """@en ;
  skos:example "For example, the relationship between a sensor and the scientific measuring Procedure via which it senses."@en ;
  schema:domainIncludes sosa:System ;
  schema:rangeIncludes sosa:Procedure ;
  owl:inverseOf sosa:implementedBy ;
  rdfs:isDefinedBy sosa-common: .

sosa:madeExecution 
  a owl:ObjectProperty ;
  rdfs:label "made execution"@en ;
  skos:definition """
  Relation between an System and an Execution it has made.
  """@en ;
  schema:domainIncludes sosa:System ;
  schema:rangeIncludes sosa:Execution ;
  owl:inverseOf sosa:madeBySystem ;
  rdfs:isDefinedBy sosa-common: .


sosa:hasSubSystem 
  a owl:ObjectProperty ;
  rdfs:label "has subsystem"@en ;
  skos:definition """
  Relation between a System and its component parts.
  """@en ;
  schema:domainIncludes sosa:System ;
  schema:rangeIncludes sosa:System ;
  rdfs:isDefinedBy sosa-common: .

sosa:isHostedBy 
  a owl:ObjectProperty ;
  rdfs:label "is hosted by"@en ;
  skos:definition """
  Relation between a Sensor, Actuator, Sampler, or Platform, and the Platform that it is mounted on or hosted by.
  """@en ;
  schema:domainIncludes sosa:System ;
  schema:domainIncludes sosa:Platform ;
  schema:rangeIncludes sosa:Platform ;
  owl:inverseOf sosa:hosts ;
  rdfs:isDefinedBy sosa-common: .

sosa:hasDeployment 
  a owl:ObjectProperty ;
  rdfs:label "has deployment"@en ;
  skos:definition """
  Relation between a System and a Deployment, recording that the System is deployed in that Deployment.
  """@en ;
  owl:inverseOf sosa:deployedSystem ;
  schema:domainIncludes sosa:System ;
  schema:rangeIncludes sosa:Deployment ;
  rdfs:isDefinedBy sosa-common: .


## Platform 

sosa:Platform 
  a owl:Class ;
  rdfs:label "Platform or Host"@en ;
  skos:prefLabel "Platform" ;
  skos:altLabel "Host" ;
  skos:definition """
  A Platform is an entity that hosts other entities, particularly Sensors, Actuators, Samplers, and other Platforms.
  """@en ;
  skos:scopeNote "The INSPIRE 'Environmental Monitoring Facility' may be implemented using SOSA by the OWL/RDFS class 'Platform'" ;
  dcterms:source <https://inspire.ec.europa.eu/id/document/tg/ef> ;
  skos:example """A post, buoy, vehicle, ship, aircraft, satellite, cell-phone, human or animal may act as platforms for (technical or biological) sensors or actuators.
  An environmental monitoring facility. 
  A platform that hosts a set of sensors. 
  A team performing a survey, where each team member would be modeled as an Observer."""@en ;
  rdfs:isDefinedBy sosa-common: .

sosa:hosts 
  a owl:ObjectProperty ;
  rdfs:label "hosts"@en ;
  skos:definition """
  Relation between a Platform and a System (Sensor, Actuator, Sampler), or Platform, hosted or mounted on it."""@en ;
  schema:domainIncludes sosa:Platform ;
  schema:rangeIncludes sosa:Platform ;
  schema:rangeIncludes sosa:System ;
  owl:inverseOf sosa:isHostedBy ;
  rdfs:isDefinedBy sosa-common: .

sosa:inDeployment 
  a owl:ObjectProperty ;
  rdfs:label "in deployment"@en ;
  skos:definition """
  Relation between a Platform and a Deployment, meaning that the deployedSystems of the Deployment are hosted on the Platform.
  """@en ;
  skos:example "For example, a relation between a buoy and a deployment of several Sensors."@en ;
  owl:inverseOf sosa:deployedOnPlatform ;
  schema:domainIncludes sosa:Platform ;
  schema:rangeIncludes sosa:Deployment ;
  rdfs:isDefinedBy sosa-common: .


## Deployment

sosa:Deployment 
  a owl:Class ;
  rdfs:label "Deployment"@en ;
  skos:definition """
  Describes the Deployment of one or more assets for a particular purpose. Deployment may be done on a Platform or Host.
  """@en ;
  skos:example "For example, a temperature Sensor deployed on a wall, or a whole network of Sensors deployed for an Observation campaign."@en ;
  rdfs:isDefinedBy sosa-common: .

sosa:deployedAsset 
  a owl:ObjectProperty ;
  rdfs:label "deployed asset"@en ;
  skos:definition """
  Relation between a Deployment and a deployed asset (System or Platform).
  """@en ;
  schema:domainIncludes sosa:Deployment ;
  schema:rangeIncludes sosa:Platform ;
  schema:rangeIncludes sosa:System ;
  rdfs:isDefinedBy sosa-common: .

sosa:deployedSystem 
  a owl:ObjectProperty ;
  rdfs:label "deployed system"@en ;
  skos:definition """
  Relation between a Deployment and a deployed System.
  """@en ;
  owl:inverseOf sosa:hasDeployment ;
  schema:domainIncludes sosa:Deployment ;
  schema:rangeIncludes sosa:System ;
  rdfs:isDefinedBy sosa-common: .

sosa:deployedOnPlatform 
  a owl:ObjectProperty ;
  rdfs:label "deployed on platform"@en ;
  skos:definition """
  Relation between a Deployment and the Platform on which the Systems are deployed.
  """@en ;
  owl:inverseOf sosa:inDeployment ;
  schema:domainIncludes sosa:Deployment ;
  schema:rangeIncludes sosa:Platform ;
  rdfs:isDefinedBy sosa-common: .

