@prefix rdf: <http://www.w3.org/1999/02/22-rdf-syntax-ns#> .
@prefix rdfs: <http://www.w3.org/2000/01/rdf-schema#> .
@prefix owl: <http://www.w3.org/2002/07/owl#> .
@prefix xsd: <http://www.w3.org/2001/XMLSchema#> .
@prefix skos: <http://www.w3.org/2004/02/skos/core#> .
@prefix dcterms: <http://purl.org/dc/terms/> .
@prefix foaf: <http://xmlns.com/foaf/0.1/>.
@prefix time: <http://www.w3.org/2006/time#> .

@prefix schema: <http://schema.org/> .

@prefix sosa: <http://www.w3.org/ns/sosa/> .
@prefix sosa-common: <http://www.w3.org/ns/sosa/common/> .
@prefix sosa-obs: <http://www.w3.org/ns/sosa/obs/> .


sosa-obs: 
  a owl:Ontology ;
  dcterms:title "Sensor, Observation, Sample, and Actuator (SOSA) Ontology - actuation module"@en ;
  dcterms:description "Observation classes and properties for the SSN Ontology."@en ;
  dcterms:creator [ a foaf:Agent ; foaf:name "W3C/OGC Spatial Data on the Web Working Group"@en ] ;
  dcterms:rights "Copyright 2024 W3C/OGC." ;
  dcterms:license <http://www.w3.org/Consortium/Legal/2015/copyright-software-and-document> ;
  dcterms:license <http://www.opengeospatial.org/ogc/Software> ;
  dcterms:created "2024-02-02"^^xsd:date ;
  owl:imports sosa-common: ;
  .

sosa:ObservableProperty 
  a owl:Class ;
  rdfs:label "Observable Property"@en ;
  skos:definition """
  An observable quality (property, characteristic) of a FeatureOfInterest.
  """@en ;
  skos:note "'Observable' means that the value can be determined through an act of Observation using an ObservationProcedure applied by a Sensor or Observer. This can be contrasted with properties whose value is assigned by some authority (e.g. price, ownership), or whose value is a consequence of some other values (e.g. rank). "@en ;
  skos:example "The height of a tree, the depth of a water body, or the temperature of a surface. "@en ;
  rdfs:isDefinedBy sosa-obs: .

sosa:isObservedBy 
  a owl:ObjectProperty ;
  rdfs:label "is observed by"@en ;
  skos:definition """
  Relation between an ObservableProperty and the Sensor able to observe it.
  """@en ;
  schema:domainIncludes sosa:ObservableProperty ;
  schema:rangeIncludes sosa:Sensor ;
  owl:inverseOf sosa:observes ;
  rdfs:isDefinedBy sosa-obs: .

sosa:wasObservedBy 
  a owl:ObjectProperty ;
  rdfs:label "was observed by"@en ;
  skos:definition """
  Relation linking a Property to the Observation or Observation Collection that observed it. 
  """@en ;
  schema:domainIncludes sosa:ObservableProperty ;
  schema:rangeIncludes sosa:Observation ;
  schema:rangeIncludes sosa:ObservationCollection ;
  owl:inverseOf sosa:observedProperty ;
  rdfs:isDefinedBy sosa-obs: .

sosa:hasProxy 
  a owl:ObjectProperty ;
  rdfs:label "has proxy"@en ;
  skos:definition """
  A relation from a Property to the Stimulus that serves as its proxy."""@en ;
  schema:domainIncludes sosa:ObservableProperty ;
  schema:rangeIncludes sosa:Stimulus ;
  owl:inverseOf sosa:isProxyFor ;
  rdfs:isDefinedBy sosa-obs: .

sosa:ObservingProcedure 
  a owl:Class ;
  rdfs:label "Observing Procedure"@en ;
  skos:definition """
  The description of steps performed in order to determine the value of an ObservableProperty by an Observer.
  """@en ;
  skos:example "A workflow, protocol, plan, algorithm, or computational method specifying how to make an observation; the description of the process utilized by an observer. This could be a chemical analysis method, a protocol for measuring an object, but could also be a checklist utilized by a human observer during a biodiversity campaign."@en ;
  skos:scopeNote "The observing procedure cannot describe a sensor instance, but it can describe the sensor type."@en ;
  rdfs:isDefinedBy sosa-obs: .

sosa:Observation 
  a owl:Class ;
  rdfs:label "Observation"@en ;
  skos:definition """
  Act of carrying out an (Observation) Procedure to estimate or calculate a value of a property of a FeatureOfInterest. Links to a Sensor to describe what made the Observation and how; links to an ObservableProperty to describe what the result is an estimate of, and to a FeatureOfInterest to detail what entity that property was associated with.
  """@en ;
  skos:scopeNote """
  An Observation concerns a single ObservableProperty of a single FeatureOfInterest. 
  Observations of multiple properties, or other combinations of Observations, may be described in an ObservationCollection. 
  
  Alternatively, applications may choose to encapsulate complexity by defining a complex property with multiple individual components, and a corresponding complex result (e.g. a vector). 
  This approach is not prohibited by the SSN Ontology, but the details are beyond the scope of SSN.
  """@en ;
  skos:example "The activity of estimating the intensity of an Earthquake using the Mercalli intensity scale is an Observation as is measuring the moment magnitude, i.e., the energy released by said earthquake."@en ;
  rdfs:isDefinedBy sosa-obs: .

sosa:relatedObservation 
  a owl:ObjectProperty ;
  rdfs:label "related observation"@en ;
  skos:definition """
  Relation to an Observation.
  """@en ;
  skos:scopeNote "This general relationship complements the specific predicates inbound to Observation. It is particularly useful to relate Observations (and collections) to other Executions (and collections)" ;
  schema:domainIncludes sosa:Observation ;
  schema:domainIncludes sosa:ObservationCollection ;
  schema:rangeIncludes sosa:Observation ;
  schema:rangeIncludes sosa:ObservationCollection ;
  owl:inverseOf sosa:observationRelatedTo ;
  rdfs:isDefinedBy sosa-obs: .

sosa:observationRelatedTo 
  a owl:ObjectProperty ;
  rdfs:label "observation related to"@en ;
  skos:definition """
  Relation of an Observation to something else.
  """@en ;
  skos:scopeNote "This general relationship complements the specific predicates outbound from Observation. It is particularly useful to relate Observations (and collections) to other Executions (and collections)" ;
  schema:domainIncludes sosa:Observation ;
  schema:domainIncludes sosa:ObservationCollection ;
  schema:rangeIncludes sosa:Observation ;
  schema:rangeIncludes sosa:ObservationCollection ;
  owl:inverseOf sosa:relatedObservation ;
  rdfs:isDefinedBy sosa-obs: .

sosa:ObservationCollection 
  a owl:Class ;
  rdfs:label "Observation Collection"@en ;
  skos:definition """
  Collection of one or more observations or observation collections, i.e. collections may be nested. 

  The following Observation properties may appear in an Observation Collection: 
  hasFeatureOfInterest , hasUltimateFeatureOfInterest , usedProcedure , madeBySensor , madeOnPlatform ,  observedProperty , phenomenonTime , resultTime , validTime , hasResult , hasSimpleResult , observationType , hasQualityMeasurement . 
  If it is present, the value of a property summarizes the values of the matching properties of the member observations, where membership is either direct or transitive through one or more member observation collections. 
  The following consistency rules apply with respect to the Observation properties listed above: 
  
  1. Where an individual Observation Collection omits a property, a member Observation (direct or transitive) MAY have any value for that property.

  2. Where an individual Observation Collection has a single value for a property, each member Observation(direct or transitive) MUST have that same value for the property - i.e. the collection is homogeneous in that property.  That property MAY then be omitted in any member Observation or Observation Collection.

  3. Where an individual Observation Collection has more than one value for a property, each member Observation (direct or transitive) MUST have a value for that property that matches one of the values for the property in the collection. 
  
  4. Where an individual Observation Collection has a value for a property that is a range or interval, each member Observation (direct or transitive) MUST have a value for that property that matches or falls within that range or interval.

  5. Where an individual Observation Collection has more than one value for a property that is a range or interval, each member Observation (direct or transitive) MUST have a value for that property that either matches or falls within one of those ranges or intervals.
  """@en ;
  skos:note """The members of a collection do not necessarily share a common value for any property. """@en ;
  rdfs:isDefinedBy sosa-obs: .

sosa:observedProperty 
  a owl:ObjectProperty ;
  rdfs:label "observed property"@en ;
  skos:definition """
  Relation linking an Observation or Observation Collection to the property that was observed. The ObservableProperty should be a property of the FeatureOfInterest (linked by hasFeatureOfInterest) of this Observation.
  """@en ;
  schema:domainIncludes sosa:Observation ;
  schema:domainIncludes sosa:ObservationCollection ;
  schema:rangeIncludes sosa:ObservableProperty ;
  owl:inverseOf sosa:wasObservedBy ;
  rdfs:isDefinedBy sosa-obs: .

sosa:resultQuality 
  a owl:ObjectProperty ;
  rdfs:label "observation result quality" ;
  skos:definition """
  Information pertaining to the data quality of the result.
  """@en ;
  skos:scopeNote """
  This instance-specific description complements the description of the observation Procedure, which provides information concerning the quality of all observations using this procedure.
  """@en ; 
  skos:note  """
  The quality of a result can be assessed following the procedures in the ISO 19157 series. Multiple measures can be provided.
  """ ;
  skos:note  """dqv:hasQualityMeasurement from the Data Quality Vocabulary is equivalent""" ;
  schema:domainIncludes sosa:Observation ;
  schema:domainIncludes sosa:ObservationCollection ;
  owl:inverseOf sosa:qualityOf ;
  rdfs:isDefinedBy sosa-obs: .

sosa:qualityOf 
  a owl:ObjectProperty ;
  rdfs:label "result quality of" ;
  skos:definition """
  Link to the observation or collection that this data quality assessment applies to.
  """@en ;
  schema:rangeIncludes sosa:Observation ;
  schema:rangeIncludes sosa:ObservationCollection ;
  owl:inverseOf sosa:resultQuality ;
  rdfs:isDefinedBy sosa-obs: .

sosa:madeBySensor 
  a owl:ObjectProperty ;
  rdfs:label "made by sensor or observer"@en ;
  skos:definition """
  Relation between an Observation and the Sensor or Observer which made the Observation.
  """@en ;
  schema:domainIncludes sosa:Observation ;
  schema:domainIncludes sosa:ObservationCollection ;
  schema:rangeIncludes sosa:Sensor ;
  owl:inverseOf sosa:madeObservation ;
  rdfs:isDefinedBy sosa-obs: .

sosa:wasOriginatedBy 
  a owl:ObjectProperty ;
  rdfs:label "was originated by"@en ;
  skos:definition """
  Relation between an Observation and the Stimulus that originated it.
  """@en ;
  schema:domainIncludes sosa:Observation ;
  schema:rangeIncludes sosa:Stimulus ;
  owl:inverseOf sosa:originated ;
  rdfs:isDefinedBy sosa-obs: .

sosa:Sensor 
  a owl:Class ;
  rdfs:label "Sensor or Observer"@en ;
  skos:altLabel "Observer"@en ;
  skos:prefLabel "Sensor"@en ;
  skos:definition """
  An identifiable entity that can generate Observations pertaining to an ObservableProperty by implementing an ObservingProcedure. Device, agent (including humans), or software (simulation) involved in, or implementing, a Procedure. Sensors respond to a stimulus, e.g., a change in the environment, or input data composed from the results of prior Observations, and generate a Result. Sensors can be hosted by Platforms."""@en ;
  skos:example "Accelerometers, gyroscopes, barometers, magnetometers, and so forth are Sensors that are typically mounted on a modern smartphone (which acts as Host or Platform). Other examples of Sensors include the human eyes."@en ;
  skos:note "Different Sensors can follow the same (reusable) observing Procedure for the creation of different Observations."@en ;
  skos:scopeNote "The Sensor is the entity instance, not the entity type. Pertaining to sensors, the Sensor would reference the explicit sensor, while the Procedure would reference the methodology utilized by that sensor type;"@en ;
  skos:note "A Sensor can be hosted by one or more Platform."@en ;
  skos:note "The Sensor is an instance of a sensor, instrument, implementation of an algorithm, or a being such as a person."@en ;
  skos:example "Accelerometers, gyroscopes, barometers, magnetometers, and so forth are Sensors that are typically mounted on a modern smart phone (which acts as Platform). Other examples of sensors include the human eyes."@en ;
  skos:note "The UML class 'Observer' from ISO 19156:2023 is implemented in SOSA by the OWL/RDFS class 'Sensor'. The class name 'Sensor' is preferred for backward compatibility with existing SOSA deployments. " ;
  rdfs:isDefinedBy sosa-obs: .

sosa:observes 
  a owl:ObjectProperty ;
  rdfs:label "observes"@en ;
  skos:definition """
  Relation between a Sensor and an ObservableProperty that it is capable of sensing.
  """@en ;
  schema:domainIncludes sosa:Sensor ;
  schema:rangeIncludes sosa:ObservableProperty ;
  owl:inverseOf sosa:isObservedBy ;
  rdfs:isDefinedBy sosa-obs: .

sosa:madeObservation 
  a owl:ObjectProperty ;
  rdfs:label "made observation"@en ;
  skos:definition """
  Relation between a Sensor and an Observation made by the Sensor.
  """@en ;
  schema:domainIncludes sosa:Sensor ;
  schema:rangeIncludes sosa:Observation ;
  owl:inverseOf sosa:madeBySensor ;
  rdfs:isDefinedBy sosa-obs: .

sosa:detects 
  a owl:ObjectProperty ;
  rdfs:label "detects"@en ;
  skos:definition """
  A relation from a Sensor to the Stimulus that the Sensor detects. 
  The Stimulus itself will be serving as a proxy for some ObservableProperty.
  """@en ;
  schema:domainIncludes sosa:Sensor ;
  schema:rangeIncludes sosa:Stimulus ;
  owl:inverseOf sosa:isDetectedBy ;
  rdfs:isDefinedBy sosa-obs: .

sosa:Stimulus 
  a owl:Class ;
  rdfs:label "Stimulus"@en ;
  skos:definition """
  An event in the real world that 'triggers' the Sensor. The properties associated to the Stimulus may be different to the eventual observed ObservableProperty. It is the event, not the object, that triggers the Sensor.
  """@en ;
  rdfs:isDefinedBy sosa-obs: .

sosa:isProxyFor 
  a owl:ObjectProperty ;
  rdfs:label "is proxy for"@en ;
  skos:definition """
  A relation from a Stimulus to the Property that the Stimulus is serving as a proxy for."""@en ;
  skos:example "For example, the expansion of quicksilver is a stimulus that serves as a proxy for some temperature property. An increase or decrease in the velocity of spinning cups on a wind sensor is serving as a proxy for the wind speed."@en ;
  schema:domainIncludes sosa:Stimulus ;
  schema:rangeIncludes sosa:ObservableProperty ;
  owl:inverseOf sosa:hasProxy ;
  rdfs:isDefinedBy sosa-obs: .

sosa:originated 
  a owl:ObjectProperty ;
  rdfs:label "originated"@en ;
  skos:definition """
  Relation between a Stimulus and the Observation that was originated by it.
  """@en ;
  schema:domainIncludes sosa:Stimulus ;
  schema:rangeIncludes sosa:Observation ;
  owl:inverseOf sosa:wasOriginatedBy ;
  rdfs:isDefinedBy sosa-obs: .

sosa:isDetectedBy 
  a owl:ObjectProperty ;
  rdfs:label "is detected by"@en ;
  skos:definition """
  A relation from a Stimulus to the Sensor that may detect it. 
  The Stimulus itself will be serving as a proxy for some ObservableProperty.
  """@en ;
  schema:domainIncludes sosa:Stimulus ;
  schema:rangeIncludes sosa:Sensor ;
  owl:inverseOf sosa:detects ;
  rdfs:isDefinedBy sosa-obs: .

## End of observation schema
## ---------------------------------------------------- ##
## additional domains and ranges for sosa-common: terms

## Utility terms 

sosa:hasMember 
  schema:domainIncludes sosa:ObservationCollection ;
  schema:rangeIncludes sosa:Observation ;
  schema:rangeIncludes sosa:ObservationCollection ;
  rdfs:isDefinedBy sosa-common: .

sosa:isMemberOf 
  schema:domainIncludes sosa:ObservationCollection ;
  schema:domainIncludes sosa:Observation ;
  schema:rangeIncludes sosa:ObservationCollection ;
  rdfs:isDefinedBy sosa-common: .


## Features of interest and Property

sosa:FeatureOfInterest 
  rdfs:isDefinedBy sosa-common: .

sosa:hasProperty 
  rdfs:isDefinedBy sosa-common: .

sosa:isFeatureOfInterestOf 
  schema:rangeIncludes sosa:Observation ;
  rdfs:isDefinedBy sosa-common: .

sosa:isUltimateFeatureOfInterestOf 
  schema:rangeIncludes sosa:Observation ;
  rdfs:isDefinedBy sosa-common: .

sosa:Property 
  rdfs:isDefinedBy sosa-common: .

sosa:PropertyOfInterest 
  rdfs:isDefinedBy sosa-common: .

sosa:isPropertyOf 
  rdfs:isDefinedBy sosa-common: .

sosa:hasProcedure 
  schema:domainIncludes sosa:ObservableProperty ;
  schema:rangeIncludes sosa:ObservingProcedure ;
  rdfs:isDefinedBy sosa-common: .

sosa:propertyFor
  schema:domainIncludes sosa:ObservableProperty ;
  schema:rangeIncludes sosa:ObservingProcedure ;
  schema:rangeIncludes sosa:Sensor ;
  rdfs:isDefinedBy sosa-common: .

sosa:forProperty 
  schema:domainIncludes sosa:ObservingProcedure ;
  schema:domainIncludes sosa:Sensor ;
  schema:rangeIncludes sosa:ObservableProperty ;
  rdfs:isDefinedBy sosa-common: .


## Procedures

sosa:Procedure 
  rdfs:isDefinedBy sosa-common: .

sosa:usedForExecution 
  schema:domainIncludes sosa:ObservingProcedure ;
  schema:rangeIncludes sosa:Observation ;
  rdfs:isDefinedBy sosa-common: .

sosa:implementedBy 
  schema:domainIncludes sosa:ObservingProcedure ;
  schema:rangeIncludes sosa:Sensor ;
  rdfs:isDefinedBy sosa-common: .

sosa:hasInput 
  schema:domainIncludes sosa:ObservingProcedure ;
  rdfs:isDefinedBy sosa-common: .

sosa:inputFor 
  schema:rangeIncludes sosa:ObservingProcedure ;
  rdfs:isDefinedBy sosa-common: .

sosa:hasOutput 
  schema:domainIncludes sosa:ObservingProcedure ;
  rdfs:isDefinedBy sosa-common: .

sosa:outputFor 
  schema:rangeIncludes sosa:ObservingProcedure ;
  rdfs:isDefinedBy sosa-common: .

## Executions

sosa:Execution 
  rdfs:isDefinedBy sosa-common: .

sosa:usedProcedure 
  schema:domainIncludes sosa:Observation ;
  schema:domainIncludes sosa:ObservationCollection ;
  schema:rangeIncludes sosa:ObservingProcedure ;
  rdfs:isDefinedBy sosa-common: .

sosa:startTime 
  schema:domainIncludes sosa:Observation ;
  schema:domainIncludes sosa:ObservationCollection ;
  rdfs:isDefinedBy sosa-common: .

sosa:resultTime 
  schema:domainIncludes sosa:Observation ;
  schema:domainIncludes sosa:ObservationCollection ;
  rdfs:isDefinedBy sosa-common: .

sosa:phenomenonTime 
  schema:domainIncludes sosa:Observation ;
  schema:domainIncludes sosa:ObservationCollection ;
  rdfs:isDefinedBy sosa-common: .

sosa:phenomenonOccurred 
  schema:rangeIncludes sosa:Observation ;
  rdfs:isDefinedBy sosa-common: .

sosa:hasFeatureOfInterest 
  schema:domainIncludes sosa:Observation ;
  schema:domainIncludes sosa:ObservationCollection ;
  rdfs:isDefinedBy sosa-common: .

sosa:hasUltimateFeatureOfInterest 
  schema:domainIncludes sosa:Observation ;
  schema:domainIncludes sosa:ObservationCollection ;
  rdfs:isDefinedBy sosa-common: .

sosa:hasInputValue 
  schema:domainIncludes sosa:Observation ;
  rdfs:isDefinedBy sosa-common: .

sosa:inputValueForExecution 
  schema:rangeIncludes sosa:Observation ;
  rdfs:isDefinedBy sosa-common: .

sosa:hasOutputValue 
  schema:domainIncludes sosa:Observation ;
  rdfs:isDefinedBy sosa-common: .

sosa:outputValueForExecution 
  schema:rangeIncludes sosa:Observation ;
  rdfs:isDefinedBy sosa-common: .



## Result 

sosa:hasResult 
  schema:domainIncludes sosa:Observation ;
  schema:domainIncludes sosa:ObservationCollection ;
  rdfs:isDefinedBy sosa-common: .

sosa:isResultOf 
  schema:rangeIncludes sosa:Observation ;
  rdfs:isDefinedBy sosa-common: .

sosa:hasSimpleResult 
  schema:domainIncludes sosa:Observation ;
  schema:domainIncludes sosa:ObservationCollection ;
  rdfs:isDefinedBy sosa-common: .


## Systems

sosa:System 
  rdfs:isDefinedBy sosa-common: .

sosa:implements 
  schema:domainIncludes sosa:Sensor ;
  schema:rangeIncludes sosa:ObservingProcedure ;
  rdfs:isDefinedBy sosa-common: .

sosa:hasSubSystem 
  schema:domainIncludes sosa:Sensor ;
  schema:rangeIncludes sosa:Sensor ;
  rdfs:isDefinedBy sosa-common: .

sosa:isSubSystemOf 
  schema:domainIncludes sosa:Sensor ;
  schema:rangeIncludes sosa:Sensor ;
  rdfs:isDefinedBy sosa-common: .

sosa:isHostedBy 
  schema:domainIncludes sosa:Sensor ;
  rdfs:isDefinedBy sosa-common: .

sosa:hasDeployment 
  schema:domainIncludes sosa:Sensor ;
  rdfs:isDefinedBy sosa-common: .

## Platform 

sosa:Platform 
  rdfs:isDefinedBy sosa-common: .

sosa:hosts 
  schema:rangeIncludes sosa:Sensor ;
  rdfs:isDefinedBy sosa-common: .

sosa:inDeployment 
  rdfs:isDefinedBy sosa-common: .

## Deployment

sosa:Deployment 
  rdfs:isDefinedBy sosa-common: .

sosa:deployedAsset 
  rdfs:isDefinedBy sosa-common: .

sosa:deployedSystem 
  schema:rangeIncludes sosa:Sensor ;
  rdfs:isDefinedBy sosa-common: .

sosa:deployedOnPlatform 
  rdfs:isDefinedBy sosa-common: .

