@prefix rdf: <http://www.w3.org/1999/02/22-rdf-syntax-ns#> .
@prefix rdfs: <http://www.w3.org/2000/01/rdf-schema#> .
@prefix owl: <http://www.w3.org/2002/07/owl#> .
@prefix xsd: <http://www.w3.org/2001/XMLSchema#> .
@prefix skos: <http://www.w3.org/2004/02/skos/core#> .
@prefix dcterms: <http://purl.org/dc/terms/> .
@prefix foaf: <http://xmlns.com/foaf/0.1/>.
@prefix time: <http://www.w3.org/2006/time#> .

@prefix schema: <http://schema.org/> .

@prefix sosa: <http://www.w3.org/ns/sosa/> .
@prefix sosa-common: <http://www.w3.org/ns/sosa/common/> .
@prefix sosa-sam: <http://www.w3.org/ns/sosa/sam/> .


sosa-sam: 
  a owl:Ontology ;
  dcterms:title "Sensor, Observation, Sample, and Actuator (SOSA) Ontology - actuation module"@en ;
  dcterms:description "Sampling classes and properties for the SSN Ontology."@en ;
  dcterms:creator [ a foaf:Agent ; foaf:name "W3C/OGC Spatial Data on the Web Working Group"@en ] ;
  dcterms:rights "Copyright 2024 W3C/OGC." ;
  dcterms:license <http://www.w3.org/Consortium/Legal/2015/copyright-software-and-document> ;
  dcterms:license <http://www.opengeospatial.org/ogc/Software> ;
  dcterms:created "2024-02-02"^^xsd:date ;
  owl:imports sosa-common: ;
  .

sosa:MaterialSample 
  a owl:Class ;
  rdfs:label "Material Sample"@en ;
  skos:definition """
  A MaterialSample is a physical, tangible Sample.
  """@en ;
  skos:example "A piece of rock, a blood sample, a water sample, etc."@en ;
  skos:note "MaterialSamples that are curated and preserved are sometimes known as 'specimens'."@en ;
  skos:note "MaterialSamples may be destroyed in connexion with the observation act or a subsequent preparation step."@en ;
  rdfs:isDefinedBy sosa-sam: .

sosa:Sample 
  a owl:Class ;
  rdfs:label "Sample"@en ;
  skos:definition """
  Feature which is intended to be representative of a FeatureOfInterest on which Observations may be made.

  A Sample is the result from an act of Sampling.
  """@en ;
  rdfs:comment "Physical samples are sometimes known as 'specimens'."@en ;
  skos:scopeNote """
  Samples are typically subsets or extracts from an entity or feature.
  Every sample is expected to (eventually) be the feature-of-interest of an Observation. 
  
  When the feature of interest cannot be observed directly, a sample of it might be used in Observations as a proxy for it. In such a case the Sample is the proximate Feature of Interest of the Observation, while the Feature of Interest of the act of Sampling (i.e. the entity that the Sample 'isSampleOf') is the ultimate Feature of Interest of the Observation.
  Samples are used in situations where observations cannot be made directly on the ultimate feature of interest, either because the entire feature cannot be observed, or because it is more convenient to use a proxy.
  Samples are thus artifacts of an observational strategy, and have no significant function outside of their role in the observation process. 
  The characteristics of the samples themselves are of little interest, except perhaps to the manager of a sampling campaign.

  A Sample is intended to sample some FatureOfInterest, so there is an expectation of at least one isSampleOf property. 
  However, in some cases the identity, and even the exact type, of the sampled feature may not be known when observations are made using the sample.
  """@en ;
  skos:example "A 'station' is a spatial sample, in the form of an identifiable locality where a sensor system or Procedure may be deployed and an observation made. In the context of the observation model, it connotes the 'world in the vicinity of the station', so the observed properties relate to the physical medium at the station, and not to any physical artifact such as a mooring, buoy, benchmark, monument, well, etc."@en ;
  skos:example "A statistical sample is often designed to be characteristic of an entire population, so that observations can be made regarding the sample that provide a good estimate of the properties of the population."@en ;
  skos:note "A transient sample, such as a ships-track or flight-line, might be identified and described, but is unlikely to be revisited exactly."@en ;
  rdfs:isDefinedBy sosa-sam: .

sosa:SampleCollection 
  a owl:Class ;
  rdfs:label "Sample Collection"@en ;
  skos:definition """
  Collection of one or more samples or sample collections, i.e. collections may be nested. 

  The following Sample properties may appear in a Sample Collection: 
  hasOriginalSample , hasSampledFeature , isSampleOf , isResultOfUsedProcedure , isResultOfMadeBySampler . 
  If it is present, the value of a property summarizes the values of the matching properties of the member samples, where membership is either direct or transitive through onw or more member sample collections. 

  The following consistency rules apply with respect to the Sample properties listed above: 
  
  1. Where an individual Sample Collection omits a property, a member Sample (direct or transitive) MAY have any value for that property.

  2. Where an individual Sample Collection has a single value for a property, each member Sample (direct or transitive) MUST have that same value for the property - i.e. the collection is homogeneous in that property.  That property MAY be omitted in any member Sample or Sample Collection.

  3. Where an individual Sample Collection has more than one value for a property, each member Sample (direct or transitive) MUST have a value for that property that matches one of the values for the property in the collection. 
  
  4. Where an individual Sample Collection has a value for a property that is a range or interval, each member Sample (direct or transitive) MUST have a value for that property that either matches or falls within that range or interval.

  5. Where an individual Sample Collection has more than one value for a property that is a range or interval, each member Sample (direct or transitive) MUST have a value for that property that either matches or falls within one of those ranges or intervals.
  """@en ;
  skos:note """
  The members of a collection do not necessarily share a common value for any property. 
  """ ;
  rdfs:isDefinedBy sosa-sam: .

sosa:Sampler 
  a owl:Class ;
  rdfs:label "Sampler"@en ;
  skos:definition """
  A device that implements a (Sampling) Procedure to create one or more samples.
  """@en ;
  skos:example "A ball mill, diamond drill, hammer, hypodermic syringe and needle, image Sensor or a soil auger can all act as sampling devices (i.e., be Samplers). However, sometimes the distinction between the Sampler and the Sensor is not evident, as they are packaged as a unit. A Sampler need not be a physical device."@en ;
  rdfs:isDefinedBy sosa-sam: .

sosa:Sampling 
  a owl:Class ;
  rdfs:label "Sampling"@en ;
  skos:definition """
  An act of Sampling carries out a sampling Procedure to create or transform one or more samples.
  """@en ;
  skos:example "Crushing a rock sample in a ball mill."@en ;
  skos:example "Digging a pit through a soil sequence."@en ;
  skos:example "Dividing a field site into quadrants."@en ;
  skos:example "Drawing blood from a patient."@en ;
  skos:example "Drilling an observation well."@en ;
  skos:example "Establishing a station for environmental monitoring."@en ;
  skos:example "Registering an image of the landscape."@en ;
  skos:example "Sieving a powder to separate the subset finer than 100-mesh."@en ;
  skos:example "Selecting a subset of a population."@en ;
  skos:example "Splitting a piece of drill-core to create two new samples."@en ;
  skos:example "Taking a diamond-drill core from a rock outcrop."@en ;
  rdfs:isDefinedBy sosa-sam: .

sosa:SamplingCollection 
  a owl:Class ;
  rdfs:label "Sampling Collection"@en ;
  skos:definition """
  Collection of one or more samplings or sampling collections, i.e. collections may be nested. 

  The following Sampling properties may appear in a Sampling Collection: 
  hasFeatureOfInterest , hasUltimateFeatureOfInterest , usedProcedure , madeBySampler , startTime , resultTime , hasResult . 
  If it is present, the value of a property summarizes the values of the matching properties of the member actuations, where membership is either direct or transitive through one or more member actuation collections. 
  The following consistency rules apply with respect to the Sampling properties listed above: 
  
  1. Where an individual Sampling Collection omits a property, a member Sampling (direct or transitive) MAY have any value for that property.

  2. Where an individual Sampling Collection has a single value for a property, each member Sampling (direct or transitive) MUST have that same value for the property - i.e. the collection is homogeneous in that property.  That property MAY then be omitted in any member Actuation or Actuation Collection.

  3. Where an individual Sampling Collection has more than one value for a property, each member Sampling (direct or transitive) MUST have a value for that property that matches one of the values for the property in the collection. 
  
  4. Where an individual Sampling Collection has a value for a property that is a range or interval, each member Sampling (direct or transitive) MUST have a value for that property that matches or falls within that range or interval.

  5. Where an individual Sampling Collection has more than one value for a property that is a range or interval, each member Sampling (direct or transitive) MUST have a value for that property that either matches or falls within one of those ranges or intervals.
  """@en ;
  skos:note """The members of a collection do not necessarily share a common value for any property."""@en ;
  rdfs:isDefinedBy sosa-sam: .

sosa:SpatialSample 
  a owl:Class ;
  rdfs:label "Spatial Sample"@en ;
  skos:definition """
  A SpatialSample is a geospatial Sample. 
  When observations are made to estimate properties of a geospatial feature, in particular where the value of a property varies within the scope of the feature, a SpatialSample is used.
  """@en ;
  skos:example "Some common names for spatial samples include: borehole, flightline, interval, lidar cloud, map horizon, microscope slide, mine level, mine, observation well, profile,  quadrat, scene, section, ship track, spot, station, swath, trajectory, traverse, etc..."@en ;
  skos:note "Depending on accessibility and on the nature of the expected property variation, the SpatialSample may be extensive in one, two or three spatial dimensions."@en ;
  rdfs:isDefinedBy sosa-sam: .

sosa:StatisticalSample 
  a owl:Class ;
  rdfs:label "Statistical Sample"@en ;
  skos:definition """
  A StatisticalSample is a statistical subset of a feature-of-interest, defined for the purpose of creating Observation(s).
  """@en ;
  skos:example "The male or female subset of a population."@en ;
  skos:note "StatisticalSamples usually apply to populations or other sets, of which certain subset may be of specific interest."@en ;
  rdfs:isDefinedBy sosa-sam: .

sosa:featureSampledBy 
  a owl:ObjectProperty ;
  rdfs:label "feature sampled by"@en ;
  skos:definition """
  Links the ultimate feature of interest to a Sample or SampleCollection - i.e. the beginning of a chain of isSampleOf relations
  """@en ;
  schema:domainIncludes sosa:FeatureOfInterest ;
  schema:rangeIncludes sosa:Sample ;
  schema:rangeIncludes sosa:SampleCollection ;
  owl:inverseOf sosa:hasSampledFeature ;
  rdfs:isDefinedBy sosa-sam: .

sosa:hasOriginalSample 
  a owl:ObjectProperty ;
  rdfs:label "has original sample"@en ;
  skos:definition """
  Link to the original sample collected from the ultimate feature of interest that is related to the context Sample or SampleCollection through a chain of isSampleOf relations.
  """@en ;
  schema:domainIncludes sosa:Sample ;
  schema:domainIncludes sosa:SampleCollection ;
  schema:rangeIncludes sosa:Sample ;
  owl:inverseOf sosa:isOriginalSampleOf ;
  rdfs:isDefinedBy sosa-sam: .

sosa:hasSample 
  a owl:ObjectProperty ;
  rdfs:label "has sample"@en ;
  skos:definition """
  Relation between a FeatureOfInterest and the Sample or SampleCollection used to represent it.
  """@en ;
  schema:domainIncludes sosa:FeatureOfInterest ;
  schema:rangeIncludes sosa:Sample ;
  owl:inverseOf sosa:isSampleOf ;
  rdfs:isDefinedBy sosa-sam: .

sosa:hasSampledFeature 
  a owl:ObjectProperty ;
  rdfs:label "has sampled feature"@en ;
  skos:definition """
  Link to the ultimate feature of interest of the context Sample or SampleCollection - i.e. the end of a chain of isSampleOf relations
  """@en ;
  schema:domainIncludes sosa:Sample ;
  schema:domainIncludes sosa:SampleCollection ;
  schema:rangeIncludes sosa:FeatureOfInterest ;
  owl:inverseOf sosa:featureSampledBy ;
  rdfs:isDefinedBy sosa-sam: .

sosa:isOriginalSampleOf 
  a owl:ObjectProperty ;
  rdfs:label "is original sample  of"@en ;
  skos:definition """
  Link the original sample collected from the ultimate feature of interest to a Sample or SampleCollection that it is related to through a chain of isSampleOf relations.
  """@en ;
  schema:domainIncludes sosa:Sample ;
  schema:rangeIncludes sosa:Sample ;
  schema:rangeIncludes sosa:SampleCollection ;
  owl:inverseOf sosa:hasOriginalSample ;
  rdfs:isDefinedBy sosa-sam: .

sosa:isResultOfMadeBySampler 
  a owl:ObjectProperty ;
  rdfs:label "is a result of made by sampler"@en ;
  skos:definition """
  Relation linking a Sample or SampleCollection to the Sampler (sampling device or entity) that made it.
  """@en ;
  schema:domainIncludes sosa:Sample ;
  schema:domainIncludes sosa:SampleCollection ;
  schema:rangeIncludes sosa:Sampler ;
  owl:inverseOf sosa:madeSamplingHasResult ;
  rdfs:isDefinedBy sosa-sam: .

sosa:isResultOfUsedProcedure 
  a owl:ObjectProperty ;
  rdfs:label "is a result of used procedure"@en ;
  skos:definition """
  Relation linking a Sample or SampleCollection to the Procedure (plan) used to make it.
  """@en ;
  schema:domainIncludes sosa:Sample ;
  schema:domainIncludes sosa:SampleCollection ;
  schema:rangeIncludes sosa:Procedure ;
  schema:rangeIncludes sosa:SamplingProcedure ;
  owl:inverseOf sosa:usedForExecutionHasResult ;
  rdfs:isDefinedBy sosa-sam: .

sosa:isSampleOf 
  a owl:ObjectProperty ;
  rdfs:label "is sample of"@en ;
  skos:definition """
  Relation from a Sample or SampleCollection to the FeatureOfInterest that it is intended to be representative of.
  """@en ;
  schema:domainIncludes sosa:Sample ;
  schema:domainIncludes sosa:SampleCollection ;
  schema:rangeIncludes sosa:FeatureOfInterest ;
  owl:inverseOf sosa:hasSample ;
  rdfs:isDefinedBy sosa-sam: .

sosa:madeBySampler 
  a owl:ObjectProperty ;
  rdfs:label "made by sampler"@en ;
  skos:definition """
  Relation linking an act of Sampling to the Sampler (sampling device or entity) that made it.
  """@en ;
  schema:domainIncludes sosa:Sampling ;
  schema:domainIncludes sosa:SamplingCollection ;
  schema:rangeIncludes sosa:Sampler ;
  owl:inverseOf sosa:madeSampling ;
  rdfs:isDefinedBy sosa-sam: .

sosa:madeSampling 
  a owl:ObjectProperty ;
  rdfs:label "made sampling"@en ;
  skos:definition """
  Relation between a Sampler (sampling device or entity) and the Sampling act it performed.
  """@en ;
  schema:domainIncludes sosa:Sampler ;
  schema:rangeIncludes sosa:Sampling ;
  owl:inverseOf sosa:madeBySampler ;
  rdfs:isDefinedBy sosa-sam: .

sosa:madeSamplingHasResult 
  a owl:ObjectProperty ;
  rdfs:label "made sampling has result"@en ;
  skos:definition """
  Relation linking a Sampler (sampling device or entity) to a Sample or SampleCollection made by it.
  """@en ;
  schema:domainIncludes sosa:Sampler ;
  schema:rangeIncludes sosa:Sample ;
  schema:rangeIncludes sosa:SampleCollection ;
  owl:inverseOf sosa:isResultOfMadeBySampler ;
  rdfs:isDefinedBy sosa-sam: .

sosa:usedForExecutionHasResult 
  a owl:ObjectProperty ;
  rdfs:label "procedure used for execution having result"@en ;
  skos:definition """
  Relation linking a Procedure (plan) to a Sample or SampleCollection used by it.
  """@en ;
  schema:domainIncludes sosa:Procedure ;
  schema:domainIncludes sosa:SamplingProcedure ;
  schema:rangeIncludes sosa:Sample ;
  schema:rangeIncludes sosa:SampleCollection ;
  owl:inverseOf sosa:isResultOfUsedProcedure ;
  rdfs:isDefinedBy sosa-sam: .

## End of sampling schema
## ---------------------------------------------------- ##
## additional domains and ranges for sosa-common: terms

## Utility terms 

sosa:hasMember 
  schema:domainIncludes sosa:SampleCollection ;
  schema:domainIncludes sosa:SamplingCollection ;
  schema:rangeIncludes sosa:Sample ;
  schema:rangeIncludes sosa:SampleCollection ;
  schema:rangeIncludes sosa:Sampling ;
  schema:rangeIncludes sosa:SamplingCollection ;
  rdfs:isDefinedBy sosa-common: .

sosa:isMemberOf 
  schema:domainIncludes sosa:Sample ;
  schema:domainIncludes sosa:SampleCollection ;
  schema:domainIncludes sosa:Sampling ;
  schema:domainIncludes sosa:SamplingCollection ;
  schema:rangeIncludes sosa:SampleCollection ;
  schema:rangeIncludes sosa:SamplingCollection ;
  rdfs:isDefinedBy sosa-common: .


## Features of interest and Property

sosa:FeatureOfInterest 
  rdfs:isDefinedBy sosa-common: .

sosa:hasProperty 
  rdfs:isDefinedBy sosa-common: .

sosa:isFeatureOfInterestOf 
  schema:rangeIncludes sosa:Sampling ;
  schema:rangeIncludes sosa:SamplingCollection ;
  rdfs:isDefinedBy sosa-common: .

sosa:isUltimateFeatureOfInterestOf 
  schema:rangeIncludes sosa:Sampling ;
  schema:rangeIncludes sosa:SamplingCollection ;
  rdfs:isDefinedBy sosa-common: .

sosa:Property 
  rdfs:isDefinedBy sosa-common: .

sosa:PropertyOfInterest 
  rdfs:isDefinedBy sosa-common: .

sosa:isPropertyOf 
  rdfs:isDefinedBy sosa-common: .

sosa:hasProcedure 
  rdfs:isDefinedBy sosa-common: .

sosa:propertyFor 
  rdfs:isDefinedBy sosa-common: .

sosa:forProperty 
  rdfs:isDefinedBy sosa-common: .


## Procedures

sosa:Procedure 
  rdfs:isDefinedBy sosa-common: .

sosa:usedForExecution 
  schema:domainIncludes sosa:SamplingProcedure ;
  schema:rangeIncludes sosa:Sampling ;
  rdfs:isDefinedBy sosa-common: .

sosa:implementedBy 
  schema:domainIncludes sosa:SamplingProcedure ;
  schema:rangeIncludes sosa:Sampler ;
  rdfs:isDefinedBy sosa-common: .

sosa:hasInput 
  schema:domainIncludes sosa:SamplingProcedure ;
  rdfs:isDefinedBy sosa-common: .

sosa:inputFor 
  schema:rangeIncludes sosa:SamplingProcedure ;
  rdfs:isDefinedBy sosa-common: .

sosa:hasOutput 
  schema:domainIncludes sosa:SamplingProcedure ;
  rdfs:isDefinedBy sosa-common: .

sosa:outputFor 
  schema:rangeIncludes sosa:SamplingProcedure ;
  rdfs:isDefinedBy sosa-common: .

## Executions

sosa:Execution 
  rdfs:isDefinedBy sosa-common: .

sosa:usedProcedure 
  schema:domainIncludes sosa:Sampling ;
  schema:domainIncludes sosa:SamplingCollection ;
  schema:rangeIncludes sosa:SamplingProcedure ;
  rdfs:isDefinedBy sosa-common: .

sosa:startTime 
  schema:domainIncludes sosa:Sampling ;
  schema:domainIncludes sosa:SamplingCollection ;
  rdfs:isDefinedBy sosa-common: .

sosa:resultTime 
  schema:domainIncludes sosa:Sampling ;
  schema:domainIncludes sosa:SamplingCollection ;
  rdfs:isDefinedBy sosa-common: .

sosa:phenomenonTime 
  schema:domainIncludes sosa:Sampling ;
  schema:domainIncludes sosa:SamplingCollection ;
  rdfs:isDefinedBy sosa-common: .

sosa:phenomenonOccurred 
  schema:rangeIncludes sosa:Sampling ;
  rdfs:isDefinedBy sosa-common: .

sosa:hasFeatureOfInterest 
  schema:domainIncludes sosa:Sampling ;
  schema:domainIncludes sosa:SamplingCollection ;
  schema:rangeIncludes sosa:Sample ;
  rdfs:isDefinedBy sosa-common: .

sosa:hasUltimateFeatureOfInterest 
  schema:domainIncludes sosa:Sampling ;
  schema:domainIncludes sosa:SamplingCollection ;
  schema:rangeIncludes sosa:Sample ;
  rdfs:isDefinedBy sosa-common: .

sosa:hasInputValue 
  schema:domainIncludes sosa:Sampling ;
  rdfs:isDefinedBy sosa-common: .

sosa:inputValueForExecution 
  schema:rangeIncludes sosa:Sampling ;
  rdfs:isDefinedBy sosa-common: .

sosa:hasOutputValue 
  schema:domainIncludes sosa:Sampling ;
  rdfs:isDefinedBy sosa-common: .

sosa:outputValueForExecution 
  schema:rangeIncludes sosa:Sampling ;
  rdfs:isDefinedBy sosa-common: .


## Result 

sosa:hasResult 
  schema:domainIncludes sosa:Sampling ;
  schema:domainIncludes sosa:SamplingCollection ;
  schema:rangeIncludes sosa:Sample ;
  rdfs:isDefinedBy sosa-common: .

sosa:isResultOf 
  schema:domainIncludes sosa:Sample ;
  schema:rangeIncludes sosa:Sampling ;
  rdfs:isDefinedBy sosa-common: .

sosa:hasSimpleResult 
  rdfs:isDefinedBy sosa-common: .


## Systems

sosa:System 
  rdfs:isDefinedBy sosa-common: .

sosa:implements 
  schema:domainIncludes sosa:Sampler ;
  schema:rangeIncludes sosa:SamplingProcedure ;
  rdfs:isDefinedBy sosa-common: .

sosa:hasSubSystem 
  schema:domainIncludes sosa:Sampler ;
  schema:rangeIncludes sosa:Sampler ;
  rdfs:isDefinedBy sosa-common: .

sosa:isSubSystemOf 
  schema:domainIncludes sosa:Sampler ;
  schema:rangeIncludes sosa:Sampler ;
  rdfs:isDefinedBy sosa-common: .

sosa:isHostedBy 
  schema:domainIncludes sosa:Sampler ;
  rdfs:isDefinedBy sosa-common: .

sosa:hasDeployment 
  schema:domainIncludes sosa:Sampler ;
  rdfs:isDefinedBy sosa-common: .

## Platform 

sosa:Platform 
  rdfs:isDefinedBy sosa-common: .

sosa:hosts 
  schema:rangeIncludes sosa:Sampler ;
  rdfs:isDefinedBy sosa-common: .

sosa:inDeployment 
  rdfs:isDefinedBy sosa-common: .

## Deployment

sosa:Deployment 
  rdfs:isDefinedBy sosa-common: .

sosa:deployedAsset 
  rdfs:isDefinedBy sosa-common: .

sosa:deployedSystem 
  schema:rangeIncludes sosa:Sampler ;
  rdfs:isDefinedBy sosa-common: .

sosa:deployedOnPlatform 
  rdfs:isDefinedBy sosa-common: .

