@prefix adms: <http://www.w3.org/ns/adms#> .
@prefix dcat: <http://www.w3.org/ns/dcat#> .
@prefix dct: <http://purl.org/dc/terms/> .
@prefix na: <http://www.opengis.net/def/metamodel/ogc-na/> .
@prefix ogcdt: <http://www.opengis.net/def/doc-type/> .
@prefix owl: <http://www.w3.org/2002/07/owl#> .
@prefix reg: <http://purl.org/linked-data/registry#> .
@prefix skos: <http://www.w3.org/2004/02/skos/core#> .
@prefix spec: <http://www.opengis.net/def/ont/modspec/> .
@prefix specrel: <http://www.opengis.net/def/ont/specrel/> .
@prefix xsd: <http://www.w3.org/2001/XMLSchema#> .
@prefix dcterms: <http://purl.org/dc/terms/> .

<http://www.opengis.net/spec/docs/20-082r2-anno> a owl:Ontology .



<http://www.opengis.net/def/docs/20-082r2> a spec:Specification ;
    dcterms:creator "Kathi Schleidt" ;
    dcterms:dateAccepted "2099-08-02"^^xsd:date ;
    dcterms:dateSubmitted "2021-07-08"^^xsd:date ;
    dcterms:identifier "http://www.opengis.net/doc/is/OMS/3.0" ;
    reg:status reg:statusValid ;
    na:doctype ogcdt:ip ;
    spec:authority "Open Geospatial Consortium" ;
    spec:class <http://www.opengis.net/spec/OMS/3.0/conf/obs-cpt>,
		<http://www.opengis.net/spec/OMS/3.0/conf/obs-core>,
		<http://www.opengis.net/spec/OMS/3.0/conf/obs-basic>,
		<http://www.opengis.net/spec/OMS/3.0/conf/obs-cpt/Observation>,
		<http://www.opengis.net/spec/OMS/3.0/conf/obs-core/AbstractObservationCharacteristics>,
		<http://www.opengis.net/spec/OMS/3.0/conf/obs-core/AbstractObservation>,
		<http://www.opengis.net/spec/OMS/3.0/conf/obs-basic/ObservationCharacteristics>,
		<http://www.opengis.net/spec/OMS/3.0/conf/obs-basic/Observation>,
		<http://www.opengis.net/spec/OMS/3.0/conf/obs-basic/ObservingCapability> ;
    spec:date "2021-12-20"^^xsd:date ;
    specrel:implementation <http://www.opengis.net/def/docs/20-082r2> ;
    skos:notation "20-082r2"^^na:doc_no ;
    skos:prefLabel "OGCÂ® Abstract Specification Topic 20 - Observations and measurements" ;
    adms:version "3.0" ;
    dcat:landingPage <http://docs.opengeospatial.org/is/20-082r2/20-082r2.html> .


<http://www.opengis.net/spec/OMS/3.0/conf/obs-cpt/Observation/Observation-sem> a spec:ConformanceTest,
        skos:Concept ;
    spec:method "Inspect the documentation of the application, schema or profile." ;
    spec:purpose "Verify that all requirements from the requirements class have been fulfilled." ;
    spec:requirement <http://www.opengis.net/spec/OMS/3.0/req/obs-cpt/Observation/Observation-sem> ;
    spec:testType spec:Capabilities ;
    skos:broader <http://www.opengis.net/spec/OMS/3.0/conf/obs-cpt/Observation> ;
    skos:broader <http://www.opengis.net/spec/OMS/3.0/conf/obs-core/AbstractObservation> ;
    skos:definition "Verify that all requirements from the requirements class have been fulfilled." ;
    skos:inScheme <http://www.opengis.net/spec/OMS/3.0> ;
    skos:prefLabel "Conformance Test http://www.opengis.net/spec/OMS/3.0/conf/obs-cpt/Observation/Observation-sem" .

<http://www.opengis.net/spec/OMS/3.0/conf/obs-cpt/Observation/resultTime-sem> a spec:ConformanceTest,
        skos:Concept ;
    spec:method "Inspect the documentation of the application, schema or profile." ;
    spec:purpose "Verify that all requirements from the requirements class have been fulfilled." ;
    spec:requirement <http://www.opengis.net/spec/OMS/3.0/req/obs-cpt/Observation/resultTime-sem> ;
    spec:testType spec:Capabilities ;
    skos:broader <http://www.opengis.net/spec/OMS/3.0/conf/obs-cpt/Observation> ;
    skos:broader <http://www.opengis.net/spec/OMS/3.0/conf/obs-core/AbstractObservationCharacteristics> ;
    skos:definition "Verify that all requirements from the requirements class have been fulfilled." ;
    skos:inScheme <http://www.opengis.net/spec/OMS/3.0> ;
    skos:prefLabel "Conformance Test http://www.opengis.net/spec/OMS/3.0/conf/obs-cpt/Observation/resultTime-sem" .

<http://www.opengis.net/spec/OMS/3.0/conf/obs-cpt/Observation/observer-sem> a spec:ConformanceTest,
        skos:Concept ;
    spec:method "Inspect the documentation of the application, schema or profile." ;
    spec:purpose "Verify that all requirements from the requirements class have been fulfilled." ;
    spec:requirement <http://www.opengis.net/spec/OMS/3.0/req/obs-cpt/Observation/observer-sem> ;
    spec:testType spec:Capabilities ;
    skos:broader <http://www.opengis.net/spec/OMS/3.0/conf/obs-cpt/Observation> ;
    skos:broader <http://www.opengis.net/spec/OMS/3.0/conf/obs-core/AbstractObservationCharacteristics> ;
    skos:definition "Verify that all requirements from the requirements class have been fulfilled." ;
    skos:inScheme <http://www.opengis.net/spec/OMS/3.0> ;
    skos:prefLabel "Conformance Test http://www.opengis.net/spec/OMS/3.0/conf/obs-cpt/Observation/observer-sem" .

<http://www.opengis.net/spec/OMS/3.0/conf/obs-core/AbstractObservation/resultTime-type> a spec:ConformanceTest,
        skos:Concept ;
    spec:method "Inspect the documentation of the application, schema or profile." ;
    spec:purpose "Verify that all requirements from the requirements class have been fulfilled." ;
    spec:requirement <http://www.opengis.net/spec/OMS/3.0/req/obs-core/AbstractObservation/resultTime-type> ;
    spec:testType spec:Capabilities ;
    skos:broader <http://www.opengis.net/spec/OMS/3.0/conf/obs-core/AbstractObservation> ;
    skos:definition "Verify that all requirements from the requirements class have been fulfilled." ;
    skos:inScheme <http://www.opengis.net/spec/OMS/3.0> ;
    skos:prefLabel "Conformance Test http://www.opengis.net/spec/OMS/3.0/conf/obs-core/AbstractObservation/resultTime-type" .

<http://www.opengis.net/spec/OMS/3.0/conf/obs-basic/ObservingCapability/ObservingCapability-sem> a spec:ConformanceTest,
        skos:Concept ;
    spec:method "Inspect the documentation of the application, schema or profile." ;
    spec:purpose "Verify that all requirements from the requirements class have been fulfilled." ;
    spec:requirement <http://www.opengis.net/spec/OMS/3.0/req/obs-basic/ObservingCapability/ObservingCapability-sem> ;
    spec:testType spec:Capabilities ;
    skos:broader <http://www.opengis.net/spec/OMS/3.0/conf/obs-basic/ObservingCapability> ;
    skos:definition "Verify that all requirements from the requirements class have been fulfilled." ;
    skos:inScheme <http://www.opengis.net/spec/OMS/3.0> ;
    skos:prefLabel "Conformance Test http://www.opengis.net/spec/OMS/3.0/conf/obs-basic/ObservingCapability/ObservingCapability-sem" .


<http://www.opengis.net/spec/OMS/3.0/req/obs-cpt> a spec:RequirementClass,
        skos:Concept ;
    spec:normativeStatement <http://www.opengis.net/spec/OMS/3.0/req/obs-cpt/Observation> ;
    skos:broader <http://www.opengis.net/spec/OMS/3.0/conf/obs-cpt> ;
    skos:definition "/req/obs-cpt" ;
    skos:inScheme <http://www.opengis.net/spec/OMS/3.0> ;
    skos:prefLabel "Requirement Class /req/obs-cpt" .

<http://www.opengis.net/spec/OMS/3.0/req/obs-core> a spec:RequirementClass,
        skos:Concept ;
    spec:normativeStatement <http://www.opengis.net/spec/OMS/3.0/req/obs-core/AbstractObservation> ;
    spec:normativeStatement <http://www.opengis.net/spec/OMS/3.0/req/obs-core/AbstractObservationCharacteristics> ;
    skos:broader <http://www.opengis.net/spec/OMS/3.0/conf/obs-core> ;
    skos:definition "/req/obs-core" ;
    skos:inScheme <http://www.opengis.net/spec/OMS/3.0> ;
    skos:prefLabel "Requirement Class /req/obs-core" .

<http://www.opengis.net/spec/OMS/3.0/req/obs-basic> a spec:RequirementClass,
        skos:Concept ;
    spec:normativeStatement <http://www.opengis.net/spec/OMS/3.0/req/obs-basic/Observation> ;
    skos:broader <http://www.opengis.net/spec/OMS/3.0/conf/obs-basic> ;
    skos:definition "/req/obs-basic" ;
    skos:inScheme <http://www.opengis.net/spec/OMS/3.0> ;
    skos:prefLabel "Requirement Class /req/obs-basic" .

<http://www.opengis.net/spec/OMS/3.0/req/obs-cpt/Observation> a spec:RequirementClass,
        skos:Concept ;
    spec:normativeStatement <http://www.opengis.net/spec/OMS/3.0/req/obs-cpt/Observation/Observation-sem> ;
    spec:normativeStatement <http://www.opengis.net/spec/OMS/3.0/req/obs-cpt/Observation/resultTime-sem> ;
    spec:normativeStatement <http://www.opengis.net/spec/OMS/3.0/req/obs-cpt/Observation/observer-sem> ;
    skos:broader <http://www.opengis.net/spec/OMS/3.0/req/obs-cpt> ;
    skos:definition "/req/obs-cpt/Observation" ;
    skos:inScheme <http://www.opengis.net/spec/OMS/3.0> ;
    skos:prefLabel "Requirement Class /req/obs-cpt/Observation" .

<http://www.opengis.net/spec/OMS/3.0/req/obs-core/AbstractObservationCharacteristics> a spec:RequirementClass,
        skos:Concept ;
    spec:normativeStatement <http://www.opengis.net/spec/OMS/3.0/req/obs-cpt/Observation/resultTime-sem> ;
    spec:normativeStatement <http://www.opengis.net/spec/OMS/3.0/req/obs-cpt/Observation/observer-sem> ;
    skos:broader <http://www.opengis.net/spec/OMS/3.0/req/obs-core> ;
    skos:definition "/req/obs-core/AbstractObservationCharacteristics" ;
    skos:inScheme <http://www.opengis.net/spec/OMS/3.0> ;
    skos:prefLabel "Requirement Class /req/obs-core/AbstractObservationCharacteristics" .

<http://www.opengis.net/spec/OMS/3.0/req/obs-core/AbstractObservation> a spec:RequirementClass,
        skos:Concept ;
    spec:normativeStatement <http://www.opengis.net/spec/OMS/3.0/req/obs-cpt/Observation/Observation-sem> ;
    spec:normativeStatement <http://www.opengis.net/spec/OMS/3.0/req/obs-core/AbstractObservationCharacteristics> ;
    skos:broader <http://www.opengis.net/spec/OMS/3.0/req/obs-core> ;
    skos:definition "/req/obs-core/AbstractObservation" ;
    skos:inScheme <http://www.opengis.net/spec/OMS/3.0> ;
    skos:prefLabel "Requirement Class /req/obs-core/AbstractObservation" .

<http://www.opengis.net/spec/OMS/3.0/req/obs-basic/ObservationCharacteristics> a spec:RequirementClass,
        skos:Concept ;
    spec:normativeStatement <http://www.opengis.net/spec/OMS/3.0/req/obs-core/AbstractObservationCharacteristics> ;
    skos:broader <http://www.opengis.net/spec/OMS/3.0/req/obs-basic> ;
    skos:definition "/req/obs-basic/ObservationCharacteristics" ;
    skos:inScheme <http://www.opengis.net/spec/OMS/3.0> ;
    skos:prefLabel "Requirement Class /req/obs-basic/ObservationCharacteristics" .

<http://www.opengis.net/spec/OMS/3.0/req/obs-basic/Observation> a spec:RequirementClass,
        skos:Concept ;
    spec:normativeStatement <http://www.opengis.net/spec/OMS/3.0/req/obs-core/AbstractObservation> ;
    skos:broader <http://www.opengis.net/spec/OMS/3.0/req/obs-basic> ;
    skos:definition "/req/obs-basic/Observation" ;
    skos:inScheme <http://www.opengis.net/spec/OMS/3.0> ;
    skos:prefLabel "Requirement Class /req/obs-basic/Observation" .

<http://www.opengis.net/spec/OMS/3.0/req/obs-basic/ObservingCapability> a spec:RequirementClass,
        skos:Concept ;
    spec:normativeStatement <http://www.opengis.net/spec/OMS/3.0/req/obs-basic/ObservationCharacteristics> ;
    spec:normativeStatement <http://www.opengis.net/spec/OMS/3.0/req/obs-basic/ObservingCapability/ObservingCapability-sem> ;
    skos:broader <http://www.opengis.net/spec/OMS/3.0/req/obs-cpt> ;
    skos:definition "/obs-basic/ObservingCapability" ;
    skos:inScheme <http://www.opengis.net/spec/OMS/3.0> ;
    skos:prefLabel "Requirement Class /obs-basic/ObservingCapability" .








<http://www.opengis.net/spec/OMS/3.0/req/obs-cpt/Observation/Observation-sem> a spec:Requirement,
        skos:Concept ;
    dcterms:description "An observation is an act carried out by an Observer to determine the value of a Property of an object (featureOfInterest) by using a Procedure; the value is provided as the result." ;
    skos:broader <http://www.opengis.net/spec/OMS/3.0/req/obs-cpt/Observation> ;
    skos:broader <http://www.opengis.net/spec/OMS/3.0/req/obs-core/AbstractObservation> ;
    skos:definition "An observation is an act carried out by an Observer to determine the value of a Property of an object (featureOfInterest) by using a Procedure; the value is provided as the result." ;
    skos:inScheme <http://www.opengis.net/spec/OMS/3.0> ;
    skos:prefLabel "Requirement: /req/obs-cpt/Observation/Observation-sem" .


<http://www.opengis.net/spec/OMS/3.0/req/obs-cpt/Observation/resultTime-sem> a spec:Requirement,
        skos:Concept ;
    dcterms:description "The instant of time when the result of the Observation became available. If the resultTime is described, this SHALL be provided by the attribute resultTime:TM_Object" ;
    skos:broader <http://www.opengis.net/spec/OMS/3.0/req/obs-cpt/Observation> ;
    skos:broader <http://www.opengis.net/spec/OMS/3.0/req/obs-core/AbstractObservationCharacteristics> ;
    skos:definition "The instant of time when the result of the Observation became available. If the resultTime is described, this SHALL be provided by the attribute resultTime:TM_Object" ;
    skos:inScheme <http://www.opengis.net/spec/OMS/3.0> ;
    skos:prefLabel "Requirement: /req/obs-cpt/Observation/resultTime-sem" .



<http://www.opengis.net/spec/OMS/3.0/req/obs-cpt/Observation/observer-sem> a spec:Requirement,
        skos:Concept ;
    dcterms:description "An Observer (ref) that is involved in the creation of this Observation. If a reference to an Observer is provided, the association with the role observer SHALL be used." ;
    skos:broader <http://www.opengis.net/spec/OMS/3.0/req/obs-cpt/Observation> ;
    skos:broader <http://www.opengis.net/spec/OMS/3.0/req/obs-core/AbstractObservationCharacteristics> ;
    skos:definition "An Observer (ref) that is involved in the creation of this Observation. If a reference to an Observer is provided, the association with the role observer SHALL be used." ;
    skos:inScheme <http://www.opengis.net/spec/OMS/3.0> ;
    skos:prefLabel "Requirement: /req/obs-cpt/Observation/observer-sem" .



<http://www.opengis.net/spec/OMS/3.0/req/obs-core/AbstractObservation/resultTime-type> a spec:Requirement,
        skos:Concept ;
    dcterms:description "If the result time of the Observation is provided, the resultTime attribute SHALL be of type TM_Instant." ;
    skos:broader <http://www.opengis.net/spec/OMS/3.0/req/obs-core/AbstractObservation> ;
    skos:definition "If the result time of the Observation is provided, the resultTime attribute SHALL be of type TM_Instant." ;
    skos:inScheme <http://www.opengis.net/spec/OMS/3.0> ;
    skos:prefLabel "Requirement: /req/obs-core/AbstractObservation/resultTime-type" .



<http://www.opengis.net/spec/OMS/3.0/req/obs-basic/ObservingCapability/ObservingCapability-sem> a spec:Requirement,
        skos:Concept ;
    dcterms:description "Information on Observation(s) that could potentially be provided." ;
    skos:broader <http://www.opengis.net/spec/OMS/3.0/req/obs-basic/ObservingCapability> ;
    skos:definition "Information on Observation(s) that could potentially be provided." ;
    skos:inScheme <http://www.opengis.net/spec/OMS/3.0> ;
    skos:prefLabel "Requirement: /req/obs-basic/ObservingCapability/ObservingCapability-sem" .

# Note: running into a dilemma as to how to nest the Conformance Classes
#     in parallel with the Requirements Classes
#Options:
#1) Use spec:conformanceTest although target is a Conformance Class, not a Conformance Test
#2) Use skos:narrower
#Currently using 2)
#
#The Requirement Classes provide skos:broader, so not adding the skos:narrower for these, assuming will be entailed


<http://www.opengis.net/spec/OMS/3.0/conf/obs-cpt> a spec:ConformanceClass,
        skos:Concept ;
    skos:definition "/conf/obs-cpt" ;
    skos:inScheme <http://www.opengis.net/spec/OMS/3.0> ;
    skos:narrower <http://www.opengis.net/spec/OMS/3.0/conf/obs-cpt/Observation> ;
    skos:prefLabel "Conformance Class /conf/obs-cpt" ;
    skos:topConceptOf <http://www.opengis.net/spec/OMS/3.0> .

<http://www.opengis.net/spec/OMS/3.0/conf/obs-core> a spec:ConformanceClass,
        skos:Concept ;
    skos:definition "/conf/obs-core" ;
    skos:inScheme <http://www.opengis.net/spec/OMS/3.0> ;
    skos:narrower <http://www.opengis.net/spec/OMS/3.0/conf/obs-core/AbstractObservation> ;
    skos:narrower <http://www.opengis.net/spec/OMS/3.0/conf/obs-core/AbstractObservationCharacteristics> ;
    skos:prefLabel "Conformance Class /conf/obs-core" ;
    skos:topConceptOf <http://www.opengis.net/spec/OMS/3.0> .


<http://www.opengis.net/spec/OMS/3.0/conf/obs-basic> a spec:ConformanceClass,
        skos:Concept ;
    skos:definition "/conf/obs-basic" ;
    skos:inScheme <http://www.opengis.net/spec/OMS/3.0> ;
    skos:narrower <http://www.opengis.net/spec/OMS/3.0/conf/obs-basic/Observation> ;
    skos:narrower <http://www.opengis.net/spec/OMS/3.0/conf/obs-basic/ObservationCharacteristics> ;
    skos:narrower <http://www.opengis.net/spec/OMS/3.0/conf/obs-basic/ObservingCapability> ;
    skos:prefLabel "Conformance Class /conf/obs-basic" ;
    skos:topConceptOf <http://www.opengis.net/spec/OMS/3.0> .


<http://www.opengis.net/spec/OMS/3.0/conf/obs-cpt/Observation> a spec:ConformanceClass,
        skos:Concept ;
    spec:conformanceTest <http://www.opengis.net/spec/OMS/3.0/conf/obs-cpt/Observation/Observation-sem> ;
    spec:conformanceTest <http://www.opengis.net/spec/OMS/3.0/conf/obs-cpt/Observation/resultTime-sem> ;
    spec:conformanceTest <http://www.opengis.net/spec/OMS/3.0/conf/obs-cpt/Observation/observer-sem> ;
    skos:definition "/conf/obs-cpt/Observation" ;
    skos:inScheme <http://www.opengis.net/spec/OMS/3.0> ;
    skos:prefLabel "Conformance Class /conf/obs-cpt/Observation" ;
    skos:topConceptOf <http://www.opengis.net/spec/OMS/3.0> .

<http://www.opengis.net/spec/OMS/3.0/conf/obs-core/AbstractObservationCharacteristics> a spec:ConformanceClass,
        skos:Concept ;
    spec:conformanceTest <http://www.opengis.net/spec/OMS/3.0/conf/obs-cpt/Observation/resultTime-sem> ;
    spec:conformanceTest <http://www.opengis.net/spec/OMS/3.0/conf/obs-cpt/Observation/observer-sem> ;
    skos:definition "/conf/obs-core/AbstractObservationCharacteristics" ;
    skos:inScheme <http://www.opengis.net/spec/OMS/3.0> ;
    skos:prefLabel "Conformance Class /conf/obs-core/AbstractObservationCharacteristics" ;
    skos:topConceptOf <http://www.opengis.net/spec/OMS/3.0> .

<http://www.opengis.net/spec/OMS/3.0/conf/obs-core/AbstractObservation> a spec:ConformanceClass,
        skos:Concept ;
    spec:conformanceTest <http://www.opengis.net/spec/OMS/3.0/conf/obs-cpt/Observation/Observation-sem> ;
    skos:narrower <http://www.opengis.net/spec/OMS/3.0/conf/obs-core/AbstractObservationCharacteristics> ;
    skos:definition "/conf/obs-core/AbstractObservation" ;
    skos:inScheme <http://www.opengis.net/spec/OMS/3.0> ;
    skos:prefLabel "Conformance Class /conf/obs-core/AbstractObservation" ;
    skos:topConceptOf <http://www.opengis.net/spec/OMS/3.0> .

<http://www.opengis.net/spec/OMS/3.0/conf/obs-basic/ObservationCharacteristics> a spec:ConformanceClass,
        skos:Concept ;
    skos:narrower <http://www.opengis.net/spec/OMS/3.0/conf/obs-core/AbstractObservationCharacteristics> ;
    skos:definition "/conf/obs-basic/ObservationCharacteristics" ;
    skos:inScheme <http://www.opengis.net/spec/OMS/3.0> ;
    skos:prefLabel "Conformance Class /conf/obs-basic/ObservationCharacteristics" ;
    skos:topConceptOf <http://www.opengis.net/spec/OMS/3.0> .

<http://www.opengis.net/spec/OMS/3.0/conf/obs-basic/Observation> a spec:ConformanceClass,
        skos:Concept ;
    skos:narrower <http://www.opengis.net/spec/OMS/3.0/conf/obs-core/AbstractObservation> ;
    skos:definition "/conf/obs-basic/Observation" ;
    skos:inScheme <http://www.opengis.net/spec/OMS/3.0> ;
    skos:prefLabel "Conformance Class /conf/obs-basic/Observation" ;
    skos:topConceptOf <http://www.opengis.net/spec/OMS/3.0> .

<http://www.opengis.net/spec/OMS/3.0/conf/obs-basic/ObservingCapability> a spec:ConformanceClass,
        skos:Concept ;
    spec:conformanceTest <http://www.opengis.net/spec/OMS/3.0/req/obs-basic/ObservingCapability/ObservingCapability-sem> ;
    skos:narrower <http://www.opengis.net/spec/OMS/3.0/conf/obs-basic/ObservationCharacteristics> ;
    skos:definition "/conf/obs-basic/ObservingCapability" ;
    skos:inScheme <http://www.opengis.net/spec/OMS/3.0> ;
    skos:prefLabel "Conformance Class /conf/obs-basic/ObservingCapability" ;
    skos:topConceptOf <http://www.opengis.net/spec/OMS/3.0> .

<http://www.opengis.net/spec/OMS/3.0> a skos:ConceptScheme ;
    dcterms:created "2021-07-08"^^xsd:date ;
    dcterms:modified "2021-07-08"^^xsd:date ;
    dcterms:source <http://www.opengis.net/def/docs/20-082r2> ;
    skos:definition "A convenience hierarchy for navigating the elements of a specification using the SKOS model" ;
    skos:hasTopConcept <http://www.opengis.net/spec/OMS/3.0/conf/obs-cpt>,
		<http://www.opengis.net/spec/OMS/3.0/conf/obs-core>,
		<http://www.opengis.net/spec/OMS/3.0/conf/obs-basic>,
		<http://www.opengis.net/spec/OMS/3.0/conf/obs-cpt/Observation>,
		<http://www.opengis.net/spec/OMS/3.0/conf/obs-core/AbstractObservationCharacteristics>,
		<http://www.opengis.net/spec/OMS/3.0/conf/obs-core/AbstractObservation>,
		<http://www.opengis.net/spec/OMS/3.0/conf/obs-basic/ObservationCharacteristics>,
		<http://www.opengis.net/spec/OMS/3.0/conf/obs-basic/Observation>,
		<http://www.opengis.net/spec/OMS/3.0/conf/obs-basic/ObservingCapability> ;
    skos:prefLabel "Specification elements for OGC 20-082r2 Observations, Measurements and Samples" .
